more helper lemmas

theories/RAs.v
@@ -1,985 +1,1 @@
-From iris.base_logic.lib Require Import gen_heap ghost_map invariants na_invariants.
-From iris.algebra Require Import auth agree dfrac csum excl gmap gmap_view gset frac_agree.
-From iris.proofmode Require Import tactics.
-From stdpp Require Import listset_nodup.
-From HypVeri Require Export lang machine.
-(* From machine_program_logic.program_logic Require Import weakestpre. *)
-
-
-  (* Context{A V W R P F:Type} `{Countable A, Countable V, Countable W, Countable R, Countable P}. *)
-
-  Class gen_VMPreG (A V W R P F: Type) (Σ:gFunctors)
-        `{Countable A, Countable V, Countable W, Countable R, Countable P} := {
-                      (* gen_num_preG_inG :> inG Σ (agreeR natO); *)
-                      gen_token_preG_inG :> inG Σ (frac_agreeR (leibnizO V));
-                      gen_mem_preG_inG :> gen_heapGpreS A W Σ;
-                      gen_reg_preG_inG :> gen_heapGpreS (R * V) W Σ;
-                      gen_tx_preG_inG :> inG Σ (authR (gmapUR V (agreeR (leibnizO P))));
-                      gen_rx_preG_inG :> inG Σ (prodR (authR (gmapUR V (agreeR (leibnizO P))))
-                                                      (optionR (gmap_viewR V (optionO (prodO natO (leibnizO V))))));
-                      (* gen_owned_preG_inG :> inG Σ (authR (gset_disjUR (leibnizO P))); *)
-                      (* gen_access_preG_inG :> inG Σ (authR (gmapUR P (prodR dfracR (csumR (agreeR unitO) (exclR unitO))))); *)
-                      gen_owned_preG_inG :> inG Σ (authR (gmapUR V
-                                    (prodR dfracR (gset_disjUR (leibnizO P)))));
-                      (* gen_access_preG_inG :> inG Σ (authR (gmapUR V *)
-                                    (* (prodR dfracR (gmapUR P (csumR (agreeR unitO) (exclR unitO)))))); *)
-                      gen_access_preG_inG :> inG Σ (authR (gmapUR V
-                                                    (prodR dfracR (gset_disjUR (leibnizO P)))));
-                      gen_trans_preG_inG :> gen_heapGpreS W (V * W* W*(gmap V (listset_nodup P))*F) Σ;
-                      gen_retri_preG_inG :> inG Σ (authR (gmapUR W (gset_disjR (leibnizO V))))
-                   }.
-
-
-  Class gen_VMG Σ := GenVMG{
-                      gen_VM_inG :> gen_VMPreG addr vmid word reg_name pid transaction_type Σ;
-                      gen_invG :> invGS Σ;
-                      gen_na_invG :> na_invG Σ;
-                      gen_nainv_name : na_inv_pool_name;
-                      gen_token_name : gname;
-                      (* gen_num_name : gname; *)
-                      gen_mem_name : gname;
-                      gen_reg_name : gname;
-                      gen_tx_name : gname;
-                      gen_rx_name : gname;
-                      gen_owned_name : gname;
-                      gen_access_name : gname;
-                      gen_trans_name : gname;
-                      gen_retri_name : gname
-                    }.
-
-Global Arguments gen_nainv_name {Σ} _.
-(* Global Arguments gen_num_name {Σ} _. *)
-Global Arguments gen_token_name {Σ} _.
-Global Arguments gen_mem_name {Σ} _.
-Global Arguments gen_reg_name {Σ} _.
-Global Arguments gen_rx_name {Σ} _.
-Global Arguments gen_tx_name {Σ} _.
-Global Arguments gen_owned_name {Σ} _.
-Global Arguments gen_access_name {Σ} _.
-Global Arguments gen_trans_name {Σ} _.
-Global Arguments gen_retri_name {Σ} _.
-
-Definition ra_TXBuffer :=
-  (authR (gmapUR vmid (agreeR (leibnizO pid)))).
-
-Definition ra_RXBuffer :=
-  (prodR ra_TXBuffer
-         (optionR (gmap_viewR vmid (optionO (prodO natO (leibnizO vmid)))))).
-Definition ra_Accessible:=
-  (* (authR (gmapUR vmid (prodR dfracR (gmapUR pid  (csumR (agreeR unitO) (exclR unitO)))))). *)
-  (* (authR (gmapUR pid (prodR dfracR (csumR (agreeR unitO) (exclR unitO))))). *)
-  (authR (gmapUR vmid (prodR dfracR (gset_disjUR (leibnizO pid))))).
-
-
-
-Definition gen_VMΣ : gFunctors :=
-  #[
-      invΣ;
-      na_invΣ;
-      (* GFunctor (agreeR natO); *)
-      GFunctor (frac_agreeR (leibnizO vmid));
-      gen_heapΣ addr word;
-      gen_heapΣ (reg_name * vmid) word;
-      GFunctor ra_TXBuffer;
-      GFunctor ra_RXBuffer;
-      GFunctor (authR (gmapUR vmid (prodR dfracR (gset_disjUR (leibnizO pid)))));
-      (* GFunctor (authR (gset_disjUR (leibnizO pid))); *)
-      GFunctor ra_Accessible;
-      gen_heapΣ word (vmid * word * word * (gmap vmid (listset_nodup pid)) * transaction_type);
-      GFunctor (authR (gmapUR word (gset_disjR (leibnizO vmid))))
-   ].
-
-Global Instance subG_gen_VMPreG {Σ}:
-  subG gen_VMΣ Σ -> gen_VMPreG addr vmid word reg_name pid transaction_type Σ.
-Proof.
-  (* hack: solve_inG does not currently unfold [subG X _] where X has more than
-     4 parameters. We have 6 (A, V, W, R, P, F). *)
-  (* set HA := gen_VMΣ. unfold gen_VMΣ in HA. *)
-  solve_inG.
-Qed.
-
-Section definitions.
-  Context `{vmG : !gen_VMG Σ}.
-  Implicit Type σ: state.
-
-
-  Definition list_of_vmids  := vec_to_list (fun_to_vec (λ v: fin vm_count, v)).
-
-  Lemma in_list_of_vmids v: In v  list_of_vmids.
-  Proof.
-    apply elem_of_list_In.
-    apply elem_of_vlookup.
-    exists v.
-    apply lookup_fun_to_vec.
-  Qed.
-
-  Definition get_token  (v:vmid) :=
-     (to_frac_agree (1/2) (v: leibnizO vmid)).
-
-  Definition get_reg_gmap σ: gmap (reg_name * vmid) word :=
-     (list_to_map (flat_map (λ v, (map (λ p, ((p.1,v),p.2)) (map_to_list (get_vm_reg_file σ v)))) (list_of_vmids))).
-
-
-  Definition get_txrx_auth_agree σ (f: mail_box -> pid) :
-    ra_TXBuffer:=
-    (● (list_to_map (map (λ v, (v,to_agree (f (get_vm_mail_box σ v)))) (list_of_vmids) )
-    )).
-
-  Definition get_tx_agree σ := get_txrx_auth_agree σ (λ p, p.1).
-
-
-  Definition get_rx_agree σ := get_txrx_auth_agree σ (λ p, p.2.1.1).
-
-
-
-  Definition get_rx_gmap σ :=
-    (Some (gmap_view_auth 1
-            ((list_to_map (map (λ v, let mb := (get_vm_mail_box σ v) in
-                                    match mb.2.2 with
-                                      | Some j => (v, (Some (0, j)))
-                                      | None => (v,None)
-                                    end) (list_of_vmids))): (gmap vmid (optionO (prodO natO (leibnizO vmid))) )))).
-
-
-  (* XXX:  seems like we have to keep resources being indexed by vmids...  *)
-
-  (* Definition get_owned_gset δ : (authR (gset_disjUR pid)) := *)
-  (*   (● (map_fold (λ (p:pid) (perm:permission) (s: gset_disjUR pid), *)
-  (*                 match perm.1 with *)
-  (*                 | Owned =>  match s with *)
-  (*                               | GSet s' => GSet (s' ∪ {[p]}) *)
-  (*                               | GSetBot => GSet ∅ *)
-  (*                             end *)
-  (*                 | Unowned => s *)
-  (*                end)  (GSet ∅) δ.2)). *)
-
-
-  (* Definition get_access_gmap δ : ra_Accessible := *)
-  (*   (●  (map_fold (λ (p:pid) (perm:permission) (s: (gmap pid (prodR dfracR (csumR (agreeR unitO) (exclR unitO))))), *)
-  (*                 match perm.2 with *)
-  (*                 | NoAccess => s *)
-  (*                 | SharedAccess => <[p:= ((DfracOwn 1), (Cinl (to_agree ())))]>s *)
-  (*                 | ExclusiveAccess => <[p:= ((DfracOwn 1),(Cinr (Excl ())))]>s *)
-  (*                end)  ∅  δ.2 )). *)
-
-  (* XXX: another attempt: *)
-
-  Definition get_owned_gmap σ : (authR (gmapUR vmid (prodR dfracR (gset_disjUR pid)))) :=
-    (● (list_to_map (map (λ v, (v, ((DfracOwn 1),
-        (GSet ((list_to_set (map (λ (p:(pid*permission)), p.1)
-           (map_to_list (filter (λ p, (is_owned p.2) = true) (get_vm_page_table σ v)))))
-                         : gset pid))))) (list_of_vmids)))).
-
-
-  (* Definition get_access_gmap σ : ra_Accessible := *)
-  (*   (● (list_to_map (map (λ v, (v, ((DfracOwn 1),(map_fold (λ (p:pid) (perm:permission) (s: (gset_disjUR pid)), *)
-  (*                 match (is_accessible perm) with *)
-  (*                 | false => s *)
-  (*                 | true => match s with *)
-  (*                                     | GSet s' => GSet (s' ∪ {[p]}) *)
-  (*                                     | GSetBot => GSet ∅ *)
-  (*                                   end *)
-  (*                end) (GSet ∅) (get_vm_page_table σ v))))) (list_of_vmids)))). *)
-
-  Definition get_access_gmap σ : ra_Accessible :=
-    (● (list_to_map (map (λ v, (v, ((DfracOwn 1),
-        (GSet ((list_to_set (map (λ (p:(pid*permission)), p.1)
-           (map_to_list (filter (λ p, (is_accessible p.2) = true) (get_vm_page_table σ v)))))
-                         : gset pid))))) (list_of_vmids)))).
-
-  (* TODO: a new exclusive ra*)
-
-  
-  Definition vec_to_gmap{A:Type}  (vec: vec A vm_count)  : gmap vmid A:=
-    (list_to_map (map (λ v, (v, (vec !!! v))) (list_of_vmids))).
-
-  (* TODO we need getters for transations.. *)
-  Definition get_trans_gmap σ : gmap word (vmid * word * word  * (gmap vmid (listset_nodup pid)) * transaction_type):=
-    list_to_map (map (λ (p:word * transaction) ,
-                      let trans := p.2 in
-                  (p.1,((((trans.1.1.1.1.1, trans.1.1.1.1.2), trans.1.1.1.2), (vec_to_gmap trans.1.2)), trans.2))
-      )  (map_to_list (get_transactions σ))).
-
-  Definition get_receivers_gmap σ : authR (gmapUR word (gset_disjR (leibnizO vmid))) :=
-    ● (list_to_map (map (λ (p:word * transaction) ,
-                      let trans := p.2 in
-                  (p.1,(GSet trans.1.1.2))) (map_to_list (get_transactions σ)))).
-
-  Definition gen_vm_interp σ: iProp Σ :=
-      (* XXX: seems like (to_agree vm_count) is not very useful ...*)
-      (* own (gen_num_name vmG) (to_agree vm_count)∗ *)
-      own (gen_token_name vmG) (get_token (get_current_vm σ)) ∗
-      ghost_map_auth (gen_mem_name vmG) 1 (get_mem σ) ∗
-      ghost_map_auth (gen_reg_name vmG) 1 (get_reg_gmap σ) ∗
-      own (gen_tx_name vmG) (get_tx_agree σ) ∗
-      own (gen_rx_name vmG) ((get_rx_agree σ), (get_rx_gmap σ) )∗
-      own (gen_owned_name vmG) (get_owned_gmap σ) ∗
-      own (gen_access_name vmG) (get_access_gmap σ) ∗
-      ghost_map_auth (gen_trans_name vmG) 1 (get_trans_gmap σ) ∗
-      own (gen_retri_name vmG) (get_receivers_gmap σ)
-    .
-
-
-  (* Definition num_agree_def (n:nat) : iProp Σ := *)
-  (*   own (gen_num_name vmG) (to_agree n). *)
-  (* Definition num_agree_aux : seal (@num_agree_def). Proof. by eexists. Qed. *)
-  (* Definition num_agree:= num_agree_aux.(unseal). *)
-  (* Definition num_agree_eq : @num_agree = @num_agree_def := num_agree_aux.(seal_eq). *)
-
-
-  Definition token_agree_def (v:vmid) : iProp Σ :=
-    own (gen_token_name vmG) (get_token v) .
-  Definition token_agree_aux : seal (@token_agree_def). Proof. by eexists. Qed.
-  Definition token_agree:= token_agree_aux.(unseal).
-  Definition token_agree_eq : @token_agree = @token_agree_def := token_agree_aux.(seal_eq).
-
-
-  Definition mem_mapsto_def (a:addr) (dq : dfrac) (w:word) : iProp Σ :=
-    (ghost_map_elem (gen_mem_name vmG) a dq w).
-    (* own (gen_mem_name vmG) (gmap_view_frag a dq (w : leibnizO word)). *)
-  Definition mem_mapsto_aux : seal (@mem_mapsto_def). Proof. by eexists. Qed.
-  Definition mem_mapsto := mem_mapsto_aux.(unseal).
-  Definition mem_mapsto_eq : @mem_mapsto = @mem_mapsto_def := mem_mapsto_aux.(seal_eq).
-
-  Definition reg_mapsto_def (r:reg_name) (i:vmid) (dq : dfrac) (w:word) : iProp Σ :=
-    (ghost_map_elem (gen_reg_name vmG) (r,i) dq w).
-    (* own (gen_reg_name vmG) (gmap_view_frag (r,i) dq (w : leibnizO word)). *)
-  Definition reg_mapsto_aux : seal (@reg_mapsto_def). Proof. by eexists. Qed.
-  Definition reg_mapsto := reg_mapsto_aux.(unseal).
-  Definition reg_mapsto_eq : @reg_mapsto = @reg_mapsto_def := reg_mapsto_aux.(seal_eq).
-
-  Definition tx_mapsto_def (i:vmid) (p:pid) : iProp Σ :=
-    own (gen_tx_name vmG) (◯ {[i := (to_agree (p: leibnizO pid))]}).
-  Definition tx_mapsto_aux : seal (@tx_mapsto_def). Proof. by eexists. Qed.
-  Definition tx_mapsto := tx_mapsto_aux.(unseal).
-  Definition tx_mapsto_eq : @tx_mapsto = @tx_mapsto_def := tx_mapsto_aux.(seal_eq).
-
-  Definition rx_mapsto_def1 (i:vmid) (p:pid) (nr : option (nat *  vmid)) : iProp Σ :=
-    match nr with
-      | Some (n, r) =>
-        own (gen_rx_name vmG) ((◯ {[i := (to_agree p)]}),
-                               (Some (gmap_view_frag i (DfracOwn 1) (Some ((n:natO), (r: leibnizO vmid))))))
-      | None =>
-        own (gen_rx_name vmG) ((◯ {[i := (to_agree p)]}),
-                               (Some (gmap_view_frag i (DfracOwn 1) None)))
-    end.
-  Definition rx_mapsto_aux1 : seal (@rx_mapsto_def1). Proof. by eexists. Qed.
-  Definition rx_mapsto1 := rx_mapsto_aux1.(unseal).
-  Definition rx_mapsto_eq1 : @rx_mapsto1 = @rx_mapsto_def1 := rx_mapsto_aux1.(seal_eq).
-
-  Definition rx_mapsto_def2 (i:vmid) (p:pid) : iProp Σ :=
-    own (gen_rx_name vmG) ((◯ {[i := (to_agree p)]}),None).
-  Definition rx_mapsto_aux2 : seal (@rx_mapsto_def2). Proof. by eexists. Qed.
-  Definition rx_mapsto2 := rx_mapsto_aux2.(unseal).
-  Definition rx_mapsto_eq2 : @rx_mapsto2 = @rx_mapsto_def2 := rx_mapsto_aux2.(seal_eq).
-
-  Definition owned_mapsto_def (i:vmid) dq (s: gset_disj pid) : iProp Σ :=
-    own (gen_owned_name vmG) (◯ {[i := (dq, s)]}).
-  (* Definition owned_mapsto_def (s: gset_disj pid) : iProp Σ := *)
-    (* own (gen_owned_name vmG) (◯ s). *)
-  Definition owned_mapsto_aux : seal (@owned_mapsto_def). Proof. by eexists. Qed.
-  Definition owned_mapsto := owned_mapsto_aux.(unseal).
-  Definition owned_mapsto_eq : @owned_mapsto = @owned_mapsto_def := owned_mapsto_aux.(seal_eq).
-
-  (* Definition access_mapsto_def (i:vmid) dq (m: gmap pid access) : iProp Σ := *)
-  (*   own (gen_access_name vmG) (◯ {[i := (dq, (map_fold (λ p a acc, *)
-  (*                                                      match a with *)
-  (*                                                        | NoAccess => acc *)
-  (*                                                        | SharedAccess => <[p:=(Cinl (to_agree ()))]>acc *)
-  (*                                                        | ExclusiveAccess => <[p:=(Cinr (Excl ()))]>acc *)
-  (*                                                      end) ∅ m))]}). *)
-  (* Definition access_mapsto_def dq (m: gmap pid access) : iProp Σ := *)
-  (*   own (gen_access_name vmG) (◯ (map_fold (λ p a acc, *)
-  (*                                                      match a with *)
-  (*                                                        | NoAccess => acc *)
-  (*                                                        | SharedAccess => <[p:=(dq, (Cinl (to_agree ())))]>acc *)
-  (*                                                        | ExclusiveAccess => <[p:=(dq, (Cinr (Excl ())))]>acc *)
-  (*                                                      end) ∅ m)). *)
-  Definition access_mapsto_def (i:vmid) dq (s: gset_disj pid) : iProp Σ :=
-    own (gen_access_name vmG) (◯ {[i := (dq,  s)]}).
-  Definition access_mapsto_aux : seal (@access_mapsto_def). Proof. by eexists. Qed.
-  Definition access_mapsto := access_mapsto_aux.(unseal).
-  Definition access_mapsto_eq : @access_mapsto = @access_mapsto_def := access_mapsto_aux.(seal_eq).
-
-  Definition trans_mapsto_def(wh : word) dq (v: vmid) (wf: word) (wt: word) (pgs : gmap vmid (listset_nodup pid)) (fid : transaction_type) : iProp Σ :=
-    own (gen_trans_name vmG) (gmap_view_frag wh dq
-                          (((((v, wf) , wt), pgs), fid): (leibnizO (vmid * word * word * (gmap vmid (listset_nodup pid)) * transaction_type)))).
-  Definition trans_mapsto_aux : seal (@trans_mapsto_def). Proof. by eexists. Qed.
-  Definition trans_mapsto := trans_mapsto_aux.(unseal).
-  Definition trans_mapsto_eq : @trans_mapsto = @trans_mapsto_def := trans_mapsto_aux.(seal_eq).
-
-  Definition retri_mapsto_def (w:word) (s: gset_disj vmid) : iProp Σ :=
-    own (gen_retri_name vmG) (◯ {[w := s]}).
-  Definition retri_mapsto_aux : seal (@retri_mapsto_def). Proof. by eexists. Qed.
-  Definition retri_mapsto := retri_mapsto_aux.(unseal).
-  Definition retri_mapsto_eq : @retri_mapsto = @retri_mapsto_def := retri_mapsto_aux.(seal_eq).
-
-End definitions.
-
-(* predicate for the number of vms *)
-(* Notation "## n" := (num_agree n) *)
-(*                         (at level 50, format "## n"): bi_scope. *)
-
-(* predicate for current vm (token) *)
-
-Notation "<< n >>" := (token_agree n)
-                        (at level 50, format "<< n >>"): bi_scope.
-
-(* point-to predicates for registers and memory *)
-Notation "r @@ i ->r{ q } w" := (reg_mapsto r i (DfracOwn q) w)
-  (at level 22, q at level 50, format "r @@ i ->r{ q } w") : bi_scope.
-Notation "r @@ i ->r w" :=
-  (reg_mapsto r i (DfracOwn 1) w) (at level 21, w at level 50) : bi_scope.
-
-Notation "a ->a{ q } w" := (mem_mapsto a (DfracOwn q) w)
-  (at level 20, q at level 50, format "a ->a{ q } w") : bi_scope.
-Notation "a ->a w" := (mem_mapsto a (DfracOwn 1) w) (at level 20) : bi_scope.
-
-(* predicates for TX and RX *)
-Notation "TX@ i := p" := (tx_mapsto i p)
-                              (at level 20, format "TX@ i := p"): bi_scope.
-Notation "RX@ i :=( p ! n , r )" := (rx_mapsto1 i p (Some (n, r)))
-                                        (at level 20, format "RX@ i :=( p ! n , r )"):bi_scope.
-Notation "RX@ i :=( p !)" := (rx_mapsto1 i p None)
-                                        (at level 20, format "RX@ i :=( p !)"):bi_scope.
-Notation "RX@ i := p " := (rx_mapsto2 i p)
-                                        (at level 20, format "RX@ i := p"):bi_scope.
-
-(* predicates for pagetables *)
-Notation "O@ i :={ q }[ s ] " := (owned_mapsto i (DfracOwn q) (GSet s))
-                                           (at level 20, format "O@ i :={ q }[ s ] "):bi_scope.
-Notation "O@ i :={ q } p" := (owned_mapsto  i (DfracOwn q) (GSet {[p]}))
-                                           (at level 20, format "O@ i :={ q } p "):bi_scope.
-
-Notation "A@ i :={ q }[ s ] " := (access_mapsto i (DfracOwn q) (GSet s))
-                                          (at level 20, format "A@ i :={ q }[ s ] "):bi_scope.
-Notation "A@ i :={ q } p " := (access_mapsto  i (DfracOwn q) (GSet {[p]}))
-                                           (at level 20, format "A@ i :={ q } p "):bi_scope.
-
-
-(* predicates for transactions *)
-Notation "w ->t{ q }( v , x , y , m , f )" := (trans_mapsto w (DfracOwn q) v x y m f)
-                                                   (at level 20, format "w ->t{ q }( v , x , y , m , f )"):bi_scope.
-Notation "w ->re[ s ]" := (retri_mapsto w (GSet s))
-                              (at level 20, format "w ->re[ s ]"):bi_scope.
-Notation "w ->re v" := (retri_mapsto w (GSet {[v]}))
-                          (at level 20, format "w ->re v"):bi_scope.
-
-Section hyp_lang_rules.
-
-  Context `{vmG :!gen_VMG Σ}.
-  Implicit Types P Q : iProp Σ.
-  Implicit Types σ : state.
-  Implicit Types a b c : addr.
-  Implicit Types r : reg_name.
-  Implicit Types w: word.
-
-
-  Lemma token_valid i1 i2 :
-   << i1 >> -∗
-      << i2 >> -∗
-      ⌜ i1 = i2 ⌝.
-  Proof.
-    rewrite token_agree_eq /token_agree_def.
-    iIntros "H1 H2".
-    iDestruct (own_valid_2  with "H1 H2") as %Hvalid.
-    rewrite /get_token in Hvalid.
-    apply frac_agree_op_valid_L in Hvalid.
-    destruct Hvalid;done.
-   Qed.
-
-    Lemma token_update i1 i2 :
-   << i1 >> -∗
-      << i1 >> ==∗
-      << i2 >> ∗ << i2 >>.
-  Proof.
-    rewrite token_agree_eq /token_agree_def /get_token.
-    rewrite -own_op.
-    iApply own_update_2.
-    rewrite - frac_agree_op.
-    pose proof (to_frac_agree_exclusive (i1: leibnizO vmid)).
-    assert (Heq:  ( 1/2 + 1/2 =  1)%Qp ).
-    { apply (bool_decide_unpack _). by compute. }
-    rewrite Heq.
-    apply (cmra_update_exclusive ).
-    rewrite -frac_agree_op.
-    unfold to_frac_agree.
-    rewrite Heq.
-    apply pair_valid.
-    split;done.
-  Qed.
-
-  (* rules for register points-to *)
-
-  Lemma reg_dupl_false r i w1 w2 :
-   r @@ i ->r w1 -∗ r @@ i ->r w2 -∗ False.
-  Proof using.
-    rewrite reg_mapsto_eq /reg_mapsto_def.
-    iIntros "Hr1 Hr2".
-    iDestruct (ghost_map_elem_valid_2 with "Hr1 Hr2") as %?.
-    destruct H.
-    apply dfrac_valid_own_r in H.
-    inversion H.
-  Qed.
-
-  Lemma reg_neq r1 r2 i j w1 w2:
-   r1 @@ i ->r w1 -∗ r2 @@ j ->r w2 -∗ ⌜ r1 <> r2 ∨ i <> j⌝.
-  Proof using.
-    iIntros "Hr1 Hr2".
-    destruct (decide (r1 = r2)).
-    destruct (decide (i = j)).
-    - simplify_eq /=.
-      iDestruct (reg_dupl_false with "Hr1 Hr2") as %[].
-    - iRight. done.
-    - iLeft. done.
-  Qed.
-
-Lemma gen_reg_valid1:
-  ∀ (σ : state) r i w,
-    (get_current_vm σ) = i ->
-    ghost_map_auth (gen_reg_name vmG) 1 (get_reg_gmap σ) -∗
-    r @@ i ->r w -∗
-          ⌜ (get_reg σ r) = Some w ⌝.
-Proof.
-  iIntros (?????) "Hσ Hr".
-  rewrite reg_mapsto_eq /reg_mapsto_def.
-  iDestruct (ghost_map_lookup with "Hσ Hr") as "%".
-  iPureIntro.
-  rewrite /get_reg /get_reg_global.
-  unfold get_reg_gmap in H0.
-  apply elem_of_list_to_map_2 in H0.
-  apply elem_of_list_In in H0.
-  apply in_flat_map in H0.
-  inversion H0; clear H0.
-  destruct H1.
-  apply in_map_iff in H1.
-  inversion H1;clear H1.
-  inversion H2;clear H2.
-  inversion H1.
-  apply elem_of_list_In in H3.
-  apply elem_of_map_to_list' in H3.
-  by simplify_eq /=.
-Qed.
-
-
-(* TODO : quite ugly... *)
-Lemma gen_reg_valid_Sep:
-  ∀ (σ : state) i (regs: gmap (reg_name * vmid) word) ,
-    (get_current_vm σ) = i ->
-    ghost_map_auth (gen_reg_name vmG) 1 (get_reg_gmap σ) -∗
-    ([∗ map] r↦w ∈ regs,  r.1 @@ r.2 ->r w)-∗
-          ([∗ map] r↦w ∈ regs, ⌜r.2 = i -> (get_reg σ r.1) = Some w ⌝).
-Proof.
-  iIntros (????) "Hσ Hregs".
-  rewrite reg_mapsto_eq /reg_mapsto_def.
-  iDestruct ((ghost_map_lookup_big regs) with "Hσ [Hregs]") as "%Hincl".
-  iApply (big_sepM_proper (λ k x, (k.1, k.2)↪[gen_reg_name vmG] x)%I).
-  intros.
-  simplify_eq.
-  f_equiv.
-  by destruct k.
-  done.
-  iApply big_sepM_pure.
-  iIntros (????).
-  rewrite /get_reg /get_reg_global.
-  apply (lookup_weaken  _ (get_reg_gmap σ) _ _) in a1;eauto.
-  apply elem_of_list_to_map_2 in a1.
-  apply elem_of_list_In in a1.
-  apply in_flat_map in a1.
-  inversion a1; clear a1.
-  destruct H0.
-  apply in_map_iff in H1.
-  inversion H1;clear H1.
-  inversion H2;clear H2.
-  inversion H1.
-  apply elem_of_list_In in H3.
-  apply elem_of_map_to_list' in H3.
-  by simplify_eq /=.
-Qed.
-
-Lemma gen_reg_valid2:
-  ∀ (σ : state) i r1 w1 r2 w2 ,
-    (get_current_vm σ) = i ->
-    r1 ≠ r2->
-    ghost_map_auth (gen_reg_name vmG) 1 (get_reg_gmap σ) -∗
-                r1 @@ i ->r w1 -∗
-                             r2 @@ i ->r w2 -∗
-           ⌜ (get_reg σ r1) = Some w1 ⌝ ∗ ⌜ (get_reg σ r2) =Some w2 ⌝.
-Proof.
-  iIntros (?????? Hneq Hi) "Hreg Hr1 Hr2".
-  iDestruct ((gen_reg_valid_Sep σ i (<[(r1,i):=w1]>{[(r2,i):=w2]}))
-               with "Hreg [Hr1 Hr2]") as "%Hreg";eauto.
-  rewrite !big_sepM_insert ?big_sepM_empty;eauto.
-  iFrame.
-  apply lookup_insert_None; split;eauto; intros P; by inversion P.
-  iPureIntro.
-  split.
-  - by apply (Hreg (r1, i) w1 (lookup_insert _ (r1, i) w1)).
-  - apply (Hreg (r2, i) w2);eauto.
-    rewrite lookup_insert_Some;right;split;
-    [intros P; inversion P; contradiction|];
-    by rewrite !lookup_insert.
- Qed.
-
-
-Lemma gen_reg_valid3:
-  ∀ (σ : state) i r1 w1 r2 w2 r3 w3 ,
-    (get_current_vm σ) = i ->
-    r1 ≠ r2->
-    r1 ≠ r3->
-    r2 ≠ r3->
-    ghost_map_auth (gen_reg_name vmG) 1 (get_reg_gmap σ) -∗
-    r1 @@ i ->r w1 -∗
-    r2 @@ i ->r w2 -∗
-    r3 @@ i ->r w3 -∗
-                ⌜ (get_reg σ r1) = Some w1 ⌝ ∗ ⌜ (get_reg σ r2) =Some w2 ⌝ ∗ ⌜ (get_reg σ r3) = Some w3⌝.
-Proof.
-  iIntros (???????? Hi Hneq1 Hneq2 Hneq3) "Hreg Hr1 Hr2 Hr3".
-  iDestruct ((gen_reg_valid_Sep σ i ({[(r1,i):=w1;(r2,i):=w2;(r3,i):=w3]}))
-               with "Hreg [Hr1 Hr2 Hr3]") as "%Hreg";eauto.
-  rewrite !big_sepM_insert ?big_sepM_empty;eauto.
-  iFrame.
-  apply lookup_insert_None; split;eauto; intros P; by inversion P.
-  apply lookup_insert_None; split;eauto.
-  apply lookup_insert_None; split;eauto; intros P; by inversion P.
-  intros P; by inversion P.
-  iPureIntro.
-  split;[|split].
-  - by apply (Hreg (r1, i) w1 (lookup_insert _ (r1, i) w1)).
-  - apply (Hreg (r2, i) w2);eauto.
-    rewrite lookup_insert_Some;right;split;
-    [intros P; inversion P; contradiction|];
-    by rewrite !lookup_insert.
-  - apply (Hreg (r3, i) w3);eauto.
-    rewrite lookup_insert_Some;right;split;
-    [intros P; inversion P; contradiction|].
-    rewrite lookup_insert_Some;right;split;
-    [intros P; inversion P; contradiction|];
-    by rewrite !lookup_insert.
-Qed.
-
-
-Lemma gen_reg_update1_global:
-  ∀ (σ : state) r i w w',
-    ghost_map_auth (gen_reg_name vmG) 1 (get_reg_gmap σ) -∗
-    r @@ i ->r w ==∗
-               ghost_map_auth (gen_reg_name vmG) 1 (<[(r,i):=w']>(get_reg_gmap σ)) ∗
-              r @@ i ->r  w'.
- Proof.
-  iIntros (?????) "Hσ Hr".
-  rewrite reg_mapsto_eq /reg_mapsto_def.
-  iDestruct (ghost_map_update w' with "Hσ Hr") as ">[Hσ Hr]".
-  iFrame.
-  done.
- Qed.
-
-
- Lemma reg_proper {m: gmap (reg_name * vmid) word}:
-([∗ map] k ↦ x ∈ m, k↪[gen_reg_name vmG] x) ⊣⊢ ([∗ map]k ↦ x ∈ m,  (k.1, k.2)↪[gen_reg_name vmG] x).
-   Proof.
-      iApply (big_sepM_proper _ (λ k x, (k.1, k.2)↪[gen_reg_name vmG] x)%I).
-      intros.
-  simpl.
-  f_equiv.
-  destruct k;done.
-Qed.
-
-
- Lemma gen_reg_update_Sep:
-  ∀ (σ : state) regs regs',
-      dom (gset (reg_name * vmid)) regs = dom (gset (reg_name * vmid )) regs' ->
-    ghost_map_auth (gen_reg_name vmG) 1 (get_reg_gmap σ) -∗
-    ([∗ map] r↦w ∈ regs,  r.1 @@ r.2 ->r w) ==∗
-               ghost_map_auth (gen_reg_name vmG) 1 (regs' ∪ (get_reg_gmap σ)) ∗
-             ([∗ map] r↦w ∈ regs',  r.1 @@ r.2 ->r w).
- Proof.
-  iIntros (????) "Hσ Hr".
-  rewrite reg_mapsto_eq /reg_mapsto_def.
-  iDestruct (ghost_map_update_big regs regs' H with "[Hσ] [Hr]") as ">[Hσ Hr]".
-  done.
-  by iApply reg_proper.
-  iModIntro.
-  rewrite reg_proper.
-  iFrame.
- Qed.
-
- Lemma gen_reg_update2_global:
-  ∀ (σ : state) r1 i1 w1 w1' r2 i2 w2 w2',
-    r1 ≠ r2 ∨ i1 ≠ i2 ->
-    ghost_map_auth (gen_reg_name vmG) 1 (get_reg_gmap σ) -∗
-     r1 @@ i1 ->r w1 -∗
-                      r2 @@ i2 ->r w2==∗
-               ghost_map_auth (gen_reg_name vmG) 1 (<[(r1,i1) := w1']> (<[(r2,i2) := w2']> (get_reg_gmap σ))) ∗
-             r1 @@ i1 ->r w1'  ∗ r2 @@ i2 ->r w2'.
- Proof.
-  iIntros (????????? Hneq) "Hreg Hr1 Hr2".
-  iDestruct ((gen_reg_update_Sep _ {[(r1,i1):=w1; (r2,i2):=w2]} {[(r1,i1):=w1'; (r2,i2):=w2']}) with "Hreg [Hr1 Hr2]")
-    as ">[Hreg Hr12]" ;eauto;[set_solver| | ].
-        rewrite !big_sepM_insert ?big_sepM_empty;eauto.
-        iFrame.
-        destruct Hneq; apply lookup_insert_None; split;eauto; intros P; by inversion P.
-        iModIntro.
-        rewrite !big_sepM_insert ?big_sepM_empty;eauto.
-        iDestruct "Hr12" as "(? & ? & _)".
-        rewrite ?insert_union_singleton_l map_union_assoc.
-        simplify_map_eq.
-        by iFrame.
-        destruct Hneq; apply lookup_insert_None; split;eauto; intros P; by inversion P.
-Qed.
-
-
- (* rules for memory points-to *)
-  Lemma mem_dupl_false a w1 w2:
-   a ->a w1 -∗ a ->a w2 -∗ False.
-  Proof using.
-    rewrite mem_mapsto_eq /mem_mapsto_def.
-    iIntros "Ha1 Ha2".
-    iDestruct (ghost_map_elem_valid_2 with "Ha1 Ha2") as %?.
-    destruct H.
-    apply dfrac_valid_own_r in H.
-    inversion H.
-  Qed.
-
-
-  Lemma mem_neq a1 a2  w1 w2:
-   a1 ->a w1 -∗ a2 ->a w2 -∗ ⌜ a1 <> a2⌝.
-  Proof using.
-    iIntros "Ha1 Ha2".
-    destruct (decide (a1 = a2)).
-    - simplify_eq /=.
-      iDestruct (mem_dupl_false with "Ha1 Ha2") as %[].
-    - done.
-  Qed.
-
-Lemma gen_mem_valid:
-  ∀ (σ : state) a w,
-    ghost_map_auth (gen_mem_name vmG) 1 (get_mem σ) -∗
-    a ->a w -∗
-          ⌜ (get_mem σ) !! a = Some w ⌝.
-Proof.
-  iIntros (???) "Hσ Ha".
-  rewrite mem_mapsto_eq /mem_mapsto_def.
-  iDestruct (ghost_map_lookup with "Hσ Ha") as "%".
-  done.
- Qed.
-
-Lemma gen_mem_valid_Sep:
-  ∀ (σ : state) mem,
-    ghost_map_auth (gen_mem_name vmG) 1 (get_mem σ) -∗
-    ([∗ map] a↦w ∈ mem,  a ->a w)-∗
-         ([∗ map] a↦w ∈ mem, ⌜ (get_mem σ) !! a = Some w ⌝).
-Proof.
-  iIntros (??) "Hσ Hmem".
-  rewrite mem_mapsto_eq /mem_mapsto_def.
-  iDestruct ((ghost_map_lookup_big mem) with "Hσ Hmem") as "%Hincl".
-  iApply big_sepM_pure.
-  iIntros (???).
-  iPureIntro.
-  apply (lookup_weaken  mem (get_mem σ) _ _ a1 Hincl) .
-Qed.
-
-Lemma gen_mem_valid2:
-  ∀ (σ : state) a1 w1 a2 w2,
-    a1 ≠ a2 ->
-    ghost_map_auth (gen_mem_name vmG) 1 (get_mem σ) -∗
-    a1 ->a w1 -∗
-    a2 ->a w2 -∗
-          ⌜ (get_mem σ) !! a1 = Some w1 ⌝ ∗ ⌜ (get_mem σ) !! a2 = Some w2 ⌝.
-Proof.
-  iIntros (????? Hneq) "Hσ Ha1 Ha2".
-  iDestruct (gen_mem_valid_Sep _ {[a1:=w1;a2:=w2]} with "Hσ [Ha1 Ha2]") as "%";eauto.
-  rewrite !big_sepM_insert ?big_sepM_empty;eauto.
-  iFrame.
-  by simplify_map_eq.
-  iPureIntro.
-  split.
-  - by apply (H a1 w1 (lookup_insert _ a1 w1)).
-  - apply (H a2 w2);eauto.
-    by simplify_map_eq.
- Qed.
-
-
-Lemma gen_mem_update1:
-  ∀ (σ : state) a w w',
-    ghost_map_auth (gen_mem_name vmG) 1 (get_mem σ) -∗
-    a ->a w ==∗
-               ghost_map_auth (gen_mem_name vmG) 1 (<[a:=w']>(get_mem σ)) ∗
-              a ->a w'.
- Proof.
-  iIntros (????) "Hσ Ha".
-  rewrite mem_mapsto_eq /mem_mapsto_def.
-  iDestruct (ghost_map_update w' with "Hσ Ha") as ">[Hσ Ha]".
-  iFrame.
-  done.
- Qed.
-
- (* rules for TX *)
-  Lemma tx_dupl i p :
-   TX@ i := p -∗ TX@ i := p ∗ TX@ i := p.
-  Proof using.
-    rewrite tx_mapsto_eq.
-    iIntros "Htx".
-    iApply own_op.
-    rewrite -auth_frag_op singleton_op.
-    rewrite agree_idemp.
-    done.
-  Qed.
-
-
-  Lemma gen_tx_valid σ i p:
-   TX@ i := p -∗ own (gen_tx_name vmG) (get_tx_agree σ) -∗ ⌜ (get_vm_mail_box σ i).1 = p ⌝.
-  Proof.
-    iIntros "Htx Hσ".
-    rewrite tx_mapsto_eq /mem_mapsto_def.
-    Admitted.
-
-
-  (* rules for RX *)
-  Lemma rx_split_some i p n (v: vmid):
-  RX@ i :=( p ! n , v)  -∗ RX@ i :=( p ! n, v)  ∗ RX@ i := p.
-  Proof using.
-    iIntros "HR".
-    rewrite rx_mapsto_eq1 rx_mapsto_eq2.
-    iApply own_op.
-    rewrite -pair_op -auth_frag_op.
-    rewrite singleton_op agree_idemp.
-    rewrite Some_op_opM.
-    simplify_eq /=.
-    done.
-  Qed.
-
-  Lemma rx_split_none i p:
-  RX@ i :=(p !) -∗ RX@ i :=(p !) ∗ RX@ i := p.
-  Proof using.
-    iIntros "HR".
-    rewrite rx_mapsto_eq1 rx_mapsto_eq2.
-    iApply own_op.
-    rewrite -pair_op -auth_frag_op.
-    rewrite singleton_op agree_idemp.
-    rewrite  Some_op_opM.
-    simplify_eq /=.
-    done.
-  Qed.
-
-  Lemma rx_dupl i p:
-   RX@i:=p -∗ RX@i:=p ∗ RX@i:=p.
-  Proof using.
-    iIntros "HR".
-    rewrite rx_mapsto_eq2.
-    iApply own_op.
-    rewrite -pair_op -auth_frag_op.
-    rewrite singleton_op agree_idemp.
-    naive_solver.
-  Qed.
-
-  (* rules for pagetables  *)
-  Lemma owned_split_set i q1 q2 (s1 s2 : gset pid):
-   s1 ## s2 -> O@i:={(q1+q2)%Qp}[(s1 ∪ s2)] -∗ O@i:={q1}[s1] ∗ O@i:={q2}[s2].
-  Proof using.
-  iIntros (Hdisj) "HO".
-  rewrite owned_mapsto_eq.
-  iApply own_op.
-  rewrite -auth_frag_op singleton_op.
-  rewrite -pair_op.
-  rewrite (gset_disj_union _ _ Hdisj).
-  naive_solver.
-  Qed.
-
-  Lemma owned_split_singleton i q1 q2 (s : gset pid) p:
-   p ∉ s -> O@i:={(q1+q2)%Qp}[(s ∪ {[p]})] -∗ O@i:={q1}[s] ∗ O@i:={q2}p.
-  Proof using.
-    iIntros (Hnotin) "HO".
-    assert (Hdisj: s ## {[p]}). { set_solver. }
-    iDestruct (owned_split_set i q1 q2 _ _ Hdisj with "HO")  as "HO'".
-    done.
-  Qed.
-
- Lemma access_split_set i q1 q2 (s1 s2 : gset pid):
-   s1 ## s2 -> A@i:={(q1+q2)%Qp}[(s1 ∪ s2)] -∗ A@i:={q1}[s1] ∗ A@i:={q2}[s2].
-  Proof using.
-  iIntros (Hdisj) "HO".
-  rewrite access_mapsto_eq.
-  iApply own_op.
-  rewrite -auth_frag_op singleton_op.
-  rewrite -pair_op.
-  rewrite (gset_disj_union _ _ Hdisj).
-  naive_solver.
-  Qed.
-
-  Lemma access_split_singleton i q1 q2 (s : gset pid) p:
-   p ∉ s -> A@i:={(q1+q2)%Qp}[(s ∪ {[p]})] -∗ A@i:={q1}[s] ∗ A@i:={q2}p.
-  Proof using.
-    iIntros (Hnotin) "HO".
-    assert (Hdisj: s ## {[p]}). { set_solver. }
-    iDestruct (access_split_set i q1 q2 _ _ Hdisj with "HO")  as "HO'".
-    done.
-  Qed.
-
-
-Lemma gen_access_valid_Set:
-  ∀ (σ : state) i q (s:gset pid),
-    own (gen_access_name vmG) (get_access_gmap σ)  -∗
-    (A@ i :={q}[s] ) -∗
-          ([∗ set]  p ∈ s, ⌜(check_access_page σ i p)= true ⌝).
-Proof.
-    iIntros (????) "Hσ Hacc".
-    rewrite access_mapsto_eq /access_mapsto_def.
-    iDestruct (own_valid_2 with "Hσ Hacc") as %Hvalid.
-    iPureIntro.
-    unfold get_access_gmap in Hvalid.
-    apply auth_both_valid_discrete in Hvalid.
-    destruct Hvalid.
-    remember (list_to_map (map
-              (λ v : vmid,
-                 (v,
-                 (DfracOwn 1,
-                 GSet
-                   (list_to_set
-                      (map (λ p : pid * permission, p.1)
-                         (map_to_list
-                            (filter (λ p : pid * permission, is_accessible p.2 = true)
-                               (get_vm_page_table σ v)))))))) list_of_vmids)) as m.
-    pose proof (lookup_included {[i := (DfracOwn q, GSet s)]} m).
-    rewrite ->H1 in H.
-    clear H1.
-    pose proof (H i).
-    clear H.
-    apply option_included in H1.
-    destruct H1.
-    simplify_map_eq.
-    destruct H.
-    destruct H.
-    destruct H.
-    apply lookup_singleton_Some in H.
-    destruct H.
-   simplify_map_eq /=.
-    destruct H1.
-   apply (elem_of_list_to_map_2 _ i x0) in H.
-   apply elem_of_list_In in H.
-   apply (in_map_iff ) in H.
-   destruct H.
-   destruct H.
-   inversion H.
-   simplify_eq /=.
-   clear H.
-   unfold set_Forall.
-   intros p Hin.
-   destruct H1.
-  - inversion H;clear H.
-      simplify_eq /=.
-      unfold check_access_page.
-      apply elem_of_list_to_set in Hin.
-      apply elem_of_list_In in Hin.
-      apply (in_map_iff _ _ p) in Hin.
-      destruct Hin.
-      destruct H.
-      rewrite <- elem_of_list_In in H1.
-      apply elem_of_map_to_list' in H1.
-      apply map_filter_lookup_Some in H1.
-      destruct H1.
-      subst p.
-      by rewrite H1 /=.
-    - apply pair_included in H.
-      destruct H;clear H.
-      apply gset_disj_included in H1.
-      unfold check_access_page.
-      assert ( p ∈ (list_to_set
-           (map (λ p : pid * permission, p.1)
-              (map_to_list (filter (λ p : pid * permission, is_accessible p.2 = true) (get_vm_page_table σ i)))): gset pid)) as Hin'.
-      { set_solver.  }
-      clear Hin;rename Hin' into Hin.
-      apply elem_of_list_to_set in Hin.
-      apply elem_of_list_In in Hin.
-      apply (in_map_iff _ _ p) in Hin.
-      destruct Hin.
-      destruct H.
-      rewrite <- elem_of_list_In in H3.
-      apply elem_of_map_to_list' in H3.
-      apply map_filter_lookup_Some in H3.
-      destruct H3.
-      subst p.
-      rewrite H3.
-      done.
-Qed.
-
-  Lemma gen_access_valid:
-  ∀ (σ : state) i q p,
-    own (gen_access_name vmG) (get_access_gmap σ)  -∗
-    (A@ i :={q}p ) -∗
-          ( ⌜(check_access_page σ i p)= true ⌝).
-  Proof.
-     iIntros (????) "Hσ Hacc".
-     iDestruct (gen_access_valid_Set _ _ _ {[p]} with "Hσ Hacc") as %->;eauto.
-     set_solver.
-  Qed.
-
-
-Lemma gen_access_valid_addr:
-  ∀ (σ : state) i q a,
-    own (gen_access_name vmG) (get_access_gmap σ)  -∗
-    (A@ i :={q} (mm_translation a) ) -∗
-          ( ⌜(check_access_addr σ i a)= true ⌝).
-Proof.
-  iIntros (????) "Haccess Hacc".
-  iDestruct (gen_access_valid σ i q (mm_translation a) with "Haccess Hacc") as %Hacc.
-  iPureIntro.
-  by unfold check_access_page.
-Qed.
-
-
-Lemma gen_access_valid_addr2:
-  ∀ (σ : state) i q s a1 a2,
-      s= {[(mm_translation a1); (mm_translation a2)]} ->
-    own (gen_access_name vmG) (get_access_gmap σ)  -∗
-    (A@ i :={q}[s] ) -∗
-          ( ⌜(check_access_addr σ i a1)= true ⌝ ∗ ⌜(check_access_addr σ i a2)= true ⌝).
-Proof.
-  iIntros (???????) "Haccess Hacc".
-  iDestruct (gen_access_valid_Set σ i q s with "Haccess Hacc") as %Hacc.
-  iPureIntro.
-  split.
-  pose proof (Hacc (mm_translation a1)).
-  apply H0.
-  set_solver.
-  pose proof (Hacc (mm_translation a2)).
-  apply H0.
-  set_solver.
-Qed.
-
-  (* TODO : gen_access_valid_Sep*)
-
-  (* rules for transactions *)
-  Lemma trans_split wh q1 q2 i wf wt m f:
-   wh ->t{(q1+q2)%Qp}(i,wf,wt,m,f) -∗  wh ->t{q1}(i,wf,wt,m,f) ∗ wh ->t{q2}(i,wf,wt,m,f).
-  Proof using.
-    iIntros "HT".
-    rewrite trans_mapsto_eq.
-    iApply own_op.
-    rewrite -gmap_view_frag_op.
-    rewrite dfrac_op_own.
-    done.
-  Qed.
-
-  Lemma retri_split_set wh (s1 s2 : gset vmid):
-   s1 ## s2 -> wh ->re[(s1 ∪ s2)] -∗ wh ->re[s1] ∗ wh ->re[s2].
-  Proof using.
-    iIntros (Hdisj) "Hre".
-    rewrite retri_mapsto_eq.
-    iApply own_op.
-    rewrite -auth_frag_op singleton_op.
-    rewrite (gset_disj_union _ _ Hdisj).
-    naive_solver.
-  Qed.
-
-  Lemma  retri_split_singleton wh (s: gset vmid) i:
-   i ∉ s -> wh ->re[(s ∪ {[i]})] -∗ wh ->re[s] ∗ wh ->re i.
-  Proof using.
-    iIntros (Hnotin) "Hr".
-    assert (Hdisj: s ## {[i]}).
-    { set_solver. }
-    iDestruct (retri_split_set wh _ _ Hdisj with "Hr")  as "Hr'".
-    done.
-  Qed.
-
-
-End hyp_lang_rules.
+From iris.base_logic.lib Require Import gen_heap ghost_map invariants na_invariants.From iris.algebra Require Import auth agree dfrac csum excl gmap gmap_view gset frac_agree.From iris.proofmode Require Import tactics.From stdpp Require Import listset_nodup.From HypVeri Require Export lang machine.(* From machine_program_logic.program_logic Require Import weakestpre. *)  (* Context{A V W R P F:Type} `{Countable A, Countable V, Countable W, Countable R, Countable P}. *)  Class gen_VMPreG (A V W R P F: Type) (Σ:gFunctors)        `{Countable A, Countable V, Countable W, Countable R, Countable P} := {                      (* gen_num_preG_inG :> inG Σ (agreeR natO); *)                      gen_token_preG_inG :> inG Σ (frac_agreeR (leibnizO V));                      gen_mem_preG_inG :> gen_heapGpreS A W Σ;                      gen_reg_preG_inG :> gen_heapGpreS (R * V) W Σ;                      gen_tx_preG_inG :> inG Σ (authR (gmapUR V (agreeR (leibnizO P))));                      gen_rx_preG_inG :> inG Σ (prodR (authR (gmapUR V (agreeR (leibnizO P))))                                                      (optionR (gmap_viewR V (optionO (prodO (leibnizO (fin page_size)) (leibnizO V))))));                      (* gen_owned_preG_inG :> inG Σ (authR (gset_disjUR (leibnizO P))); *)                      (* gen_access_preG_inG :> inG Σ (authR (gmapUR P (prodR dfracR (csumR (agreeR unitO) (exclR unitO))))); *)                      gen_owned_preG_inG :> inG Σ (authR (gmapUR V                                    (prodR dfracR (gset_disjUR (leibnizO P)))));                      (* gen_access_preG_inG :> inG Σ (authR (gmapUR V *)                                    (* (prodR dfracR (gmapUR P (csumR (agreeR unitO) (exclR unitO)))))); *)                      gen_access_preG_inG :> inG Σ (authR (gmapUR V                                                    (prodR dfracR (gset_disjUR (leibnizO P)))));                      gen_trans_preG_inG :> gen_heapGpreS W (V * W* W*(gmap V (listset_nodup P))*F) Σ;                      gen_retri_preG_inG :> inG Σ (authR (gmapUR W (gset_disjR (leibnizO V))))                   }.  Class gen_VMG Σ := GenVMG{                      gen_VM_inG :> gen_VMPreG addr vmid word reg_name pid transaction_type Σ;                      gen_invG :> invGS Σ;                      gen_na_invG :> na_invG Σ;                      gen_nainv_name : na_inv_pool_name;                      gen_token_name : gname;                      (* gen_num_name : gname; *)                      gen_mem_name : gname;                      gen_reg_name : gname;                      gen_tx_name : gname;                      gen_rx_name : gname;                      gen_owned_name : gname;                      gen_access_name : gname;                      gen_trans_name : gname;                      gen_retri_name : gname                    }.Global Arguments gen_nainv_name {Σ} _.(* Global Arguments gen_num_name {Σ} _. *)Global Arguments gen_token_name {Σ} _.Global Arguments gen_mem_name {Σ} _.Global Arguments gen_reg_name {Σ} _.Global Arguments gen_rx_name {Σ} _.Global Arguments gen_tx_name {Σ} _.Global Arguments gen_owned_name {Σ} _.Global Arguments gen_access_name {Σ} _.Global Arguments gen_trans_name {Σ} _.Global Arguments gen_retri_name {Σ} _.Definition ra_TXBuffer :=  (authR (gmapUR vmid (agreeR (leibnizO pid)))).Definition ra_RXBuffer :=  (prodR ra_TXBuffer         (optionR (gmap_viewR vmid (optionO (prodO (leibnizO (fin page_size)) (leibnizO vmid)))))).Definition ra_Accessible:=  (* (authR (gmapUR vmid (prodR dfracR (gmapUR pid  (csumR (agreeR unitO) (exclR unitO)))))). *)  (* (authR (gmapUR pid (prodR dfracR (csumR (agreeR unitO) (exclR unitO))))). *)  (authR (gmapUR vmid (prodR dfracR (gset_disjUR (leibnizO pid))))).Definition gen_VMΣ : gFunctors :=  #[      invΣ;      na_invΣ;      (* GFunctor (agreeR natO); *)      GFunctor (frac_agreeR (leibnizO vmid));      gen_heapΣ addr word;      gen_heapΣ (reg_name * vmid) word;      GFunctor ra_TXBuffer;      GFunctor ra_RXBuffer;      GFunctor (authR (gmapUR vmid (prodR dfracR (gset_disjUR (leibnizO pid)))));      (* GFunctor (authR (gset_disjUR (leibnizO pid))); *)      GFunctor ra_Accessible;      gen_heapΣ word (vmid * word * word * (gmap vmid (listset_nodup pid)) * transaction_type);      GFunctor (authR (gmapUR word (gset_disjR (leibnizO vmid))))   ].Global Instance subG_gen_VMPreG {Σ}:  subG gen_VMΣ Σ -> gen_VMPreG addr vmid word reg_name pid transaction_type Σ.Proof.  (* hack: solve_inG does not currently unfold [subG X _] where X has more than     4 parameters. We have 6 (A, V, W, R, P, F). *)  (* set HA := gen_VMΣ. unfold gen_VMΣ in HA. *)  solve_inG.Qed.Section definitions.  Context `{vmG : !gen_VMG Σ}.  Implicit Type σ: state.  Definition list_of_vmids  := vec_to_list (fun_to_vec (λ v: fin vm_count, v)).  Lemma in_list_of_vmids v: In v  list_of_vmids.  Proof.    apply elem_of_list_In.    apply elem_of_vlookup.    exists v.    apply lookup_fun_to_vec.  Qed.  Definition get_token  (v:vmid) :=     (to_frac_agree (1/2) (v: leibnizO vmid)).  Definition get_reg_gmap σ: gmap (reg_name * vmid) word :=     (list_to_map (flat_map (λ v, (map (λ p, ((p.1,v),p.2)) (map_to_list (get_vm_reg_file σ v)))) (list_of_vmids))).  Definition get_txrx_auth_agree σ (f: mail_box -> pid) :    ra_TXBuffer:=    (● (list_to_map (map (λ v, (v,to_agree (f (get_vm_mail_box σ v)))) (list_of_vmids) )    )).  Definition get_tx_agree σ := get_txrx_auth_agree σ (λ p, p.1).  Definition get_rx_agree σ := get_txrx_auth_agree σ (λ p, p.2.1).  Definition get_rx_gmap σ :=    (Some (gmap_view_auth 1            ((list_to_map (map (λ v, let mb := (get_vm_mail_box σ v) in                                    match mb.2.2 with                                      | Some (l, j) => (v, (Some ( l, j)))                                      | None => (v,None)                                    end) (list_of_vmids))): (gmap vmid (optionO (prodO (leibnizO (fin page_size)) (leibnizO vmid))) )))).  (* XXX:  seems like we have to keep resources being indexed by vmids...  *)  (* Definition get_owned_gset δ : (authR (gset_disjUR pid)) := *)  (*   (● (map_fold (λ (p:pid) (perm:permission) (s: gset_disjUR pid), *)  (*                 match perm.1 with *)  (*                 | Owned =>  match s with *)  (*                               | GSet s' => GSet (s' ∪ {[p]}) *)  (*                               | GSetBot => GSet ∅ *)  (*                             end *)  (*                 | Unowned => s *)  (*                end)  (GSet ∅) δ.2)). *)  (* Definition get_access_gmap δ : ra_Accessible := *)  (*   (●  (map_fold (λ (p:pid) (perm:permission) (s: (gmap pid (prodR dfracR (csumR (agreeR unitO) (exclR unitO))))), *)  (*                 match perm.2 with *)  (*                 | NoAccess => s *)  (*                 | SharedAccess => <[p:= ((DfracOwn 1), (Cinl (to_agree ())))]>s *)  (*                 | ExclusiveAccess => <[p:= ((DfracOwn 1),(Cinr (Excl ())))]>s *)  (*                end)  ∅  δ.2 )). *)  (* XXX: another attempt: *)  Definition get_owned_gmap σ : (authR (gmapUR vmid (prodR dfracR (gset_disjUR pid)))) :=    (● (list_to_map (map (λ v, (v, ((DfracOwn 1),        (GSet ((list_to_set (map (λ (p:(pid*permission)), p.1)           (map_to_list (filter (λ p, (is_owned p.2) = true) (get_vm_page_table σ v)))))                         : gset pid))))) (list_of_vmids)))).  (* Definition get_access_gmap σ : ra_Accessible := *)  (*   (● (list_to_map (map (λ v, (v, ((DfracOwn 1),(map_fold (λ (p:pid) (perm:permission) (s: (gset_disjUR pid)), *)  (*                 match (is_accessible perm) with *)  (*                 | false => s *)  (*                 | true => match s with *)  (*                                     | GSet s' => GSet (s' ∪ {[p]}) *)  (*                                     | GSetBot => GSet ∅ *)  (*                                   end *)  (*                end) (GSet ∅) (get_vm_page_table σ v))))) (list_of_vmids)))). *)  Definition get_access_gmap σ : ra_Accessible :=    (● (list_to_map (map (λ v, (v, ((DfracOwn 1),        (GSet ((list_to_set (map (λ (p:(pid*permission)), p.1)           (map_to_list (filter (λ p, (is_accessible p.2) = true) (get_vm_page_table σ v)))))                         : gset pid))))) (list_of_vmids)))).  (* TODO: a new exclusive ra*)    Definition vec_to_gmap{A:Type}  (vec: vec A vm_count)  : gmap vmid A:=    (list_to_map (map (λ v, (v, (vec !!! v))) (list_of_vmids))).  (* TODO we need getters for transations.. *)  Definition get_trans_gmap σ : gmap word (vmid * word * word  * (gmap vmid (listset_nodup pid)) * transaction_type):=    list_to_map (map (λ (p:word * transaction) ,                      let trans := p.2 in                  (p.1,((((trans.1.1.1.1.1, trans.1.1.1.1.2), trans.1.1.1.2), (vec_to_gmap trans.1.2)), trans.2))      )  (map_to_list (get_transactions σ))).  Definition get_receivers_gmap σ : authR (gmapUR word (gset_disjR (leibnizO vmid))) :=    ● (list_to_map (map (λ (p:word * transaction) ,                      let trans := p.2 in                  (p.1,(GSet trans.1.1.2))) (map_to_list (get_transactions σ)))).  Definition gen_vm_interp σ: iProp Σ :=      (* XXX: seems like (to_agree vm_count) is not very useful ...*)      (* own (gen_num_name vmG) (to_agree vm_count)∗ *)      own (gen_token_name vmG) (get_token (get_current_vm σ)) ∗      ghost_map_auth (gen_mem_name vmG) 1 (get_mem σ) ∗      ghost_map_auth (gen_reg_name vmG) 1 (get_reg_gmap σ) ∗      own (gen_tx_name vmG) (get_tx_agree σ) ∗      own (gen_rx_name vmG) ((get_rx_agree σ), (get_rx_gmap σ) )∗      own (gen_owned_name vmG) (get_owned_gmap σ) ∗      own (gen_access_name vmG) (get_access_gmap σ) ∗      ghost_map_auth (gen_trans_name vmG) 1 (get_trans_gmap σ) ∗      own (gen_retri_name vmG) (get_receivers_gmap σ)    .  (* Definition num_agree_def (n:nat) : iProp Σ := *)  (*   own (gen_num_name vmG) (to_agree n). *)  (* Definition num_agree_aux : seal (@num_agree_def). Proof. by eexists. Qed. *)  (* Definition num_agree:= num_agree_aux.(unseal). *)  (* Definition num_agree_eq : @num_agree = @num_agree_def := num_agree_aux.(seal_eq). *)  Definition token_agree_def (v:vmid) : iProp Σ :=    own (gen_token_name vmG) (get_token v) .  Definition token_agree_aux : seal (@token_agree_def). Proof. by eexists. Qed.  Definition token_agree:= token_agree_aux.(unseal).  Definition token_agree_eq : @token_agree = @token_agree_def := token_agree_aux.(seal_eq).  Definition mem_mapsto_def (a:addr) (dq : dfrac) (w:word) : iProp Σ :=    (ghost_map_elem (gen_mem_name vmG) a dq w).    (* own (gen_mem_name vmG) (gmap_view_frag a dq (w : leibnizO word)). *)  Definition mem_mapsto_aux : seal (@mem_mapsto_def). Proof. by eexists. Qed.  Definition mem_mapsto := mem_mapsto_aux.(unseal).  Definition mem_mapsto_eq : @mem_mapsto = @mem_mapsto_def := mem_mapsto_aux.(seal_eq).  Definition reg_mapsto_def (r:reg_name) (i:vmid) (dq : dfrac) (w:word) : iProp Σ :=    (ghost_map_elem (gen_reg_name vmG) (r,i) dq w).    (* own (gen_reg_name vmG) (gmap_view_frag (r,i) dq (w : leibnizO word)). *)  Definition reg_mapsto_aux : seal (@reg_mapsto_def). Proof. by eexists. Qed.  Definition reg_mapsto := reg_mapsto_aux.(unseal).  Definition reg_mapsto_eq : @reg_mapsto = @reg_mapsto_def := reg_mapsto_aux.(seal_eq).  Definition tx_mapsto_def (i:vmid) (p:pid) : iProp Σ :=    own (gen_tx_name vmG) (◯ {[i := (to_agree (p: leibnizO pid))]}).  Definition tx_mapsto_aux : seal (@tx_mapsto_def). Proof. by eexists. Qed.  Definition tx_mapsto := tx_mapsto_aux.(unseal).  Definition tx_mapsto_eq : @tx_mapsto = @tx_mapsto_def := tx_mapsto_aux.(seal_eq).  Definition rx_mapsto_def1 (i:vmid) (p:pid) (nr : option (fin page_size *  vmid)) : iProp Σ :=    match nr with      | Some (n, r) =>        own (gen_rx_name vmG) ((◯ {[i := (to_agree p)]}),                               (Some (gmap_view_frag i (DfracOwn 1) (Some ((n:(leibnizO (fin page_size))), (r: leibnizO vmid))))))      | None =>        own (gen_rx_name vmG) ((◯ {[i := (to_agree p)]}),                               (Some (gmap_view_frag i (DfracOwn 1) None)))    end.  Definition rx_mapsto_aux1 : seal (@rx_mapsto_def1). Proof. by eexists. Qed.  Definition rx_mapsto1 := rx_mapsto_aux1.(unseal).  Definition rx_mapsto_eq1 : @rx_mapsto1 = @rx_mapsto_def1 := rx_mapsto_aux1.(seal_eq).  Definition rx_mapsto_def2 (i:vmid) (p:pid) : iProp Σ :=    own (gen_rx_name vmG) ((◯ {[i := (to_agree p)]}),None).  Definition rx_mapsto_aux2 : seal (@rx_mapsto_def2). Proof. by eexists. Qed.  Definition rx_mapsto2 := rx_mapsto_aux2.(unseal).  Definition rx_mapsto_eq2 : @rx_mapsto2 = @rx_mapsto_def2 := rx_mapsto_aux2.(seal_eq).  Definition owned_mapsto_def (i:vmid) dq (s: gset_disj pid) : iProp Σ :=    own (gen_owned_name vmG) (◯ {[i := (dq, s)]}).  (* Definition owned_mapsto_def (s: gset_disj pid) : iProp Σ := *)    (* own (gen_owned_name vmG) (◯ s). *)  Definition owned_mapsto_aux : seal (@owned_mapsto_def). Proof. by eexists. Qed.  Definition owned_mapsto := owned_mapsto_aux.(unseal).  Definition owned_mapsto_eq : @owned_mapsto = @owned_mapsto_def := owned_mapsto_aux.(seal_eq).  (* Definition access_mapsto_def (i:vmid) dq (m: gmap pid access) : iProp Σ := *)  (*   own (gen_access_name vmG) (◯ {[i := (dq, (map_fold (λ p a acc, *)  (*                                                      match a with *)  (*                                                        | NoAccess => acc *)  (*                                                        | SharedAccess => <[p:=(Cinl (to_agree ()))]>acc *)  (*                                                        | ExclusiveAccess => <[p:=(Cinr (Excl ()))]>acc *)  (*                                                      end) ∅ m))]}). *)  (* Definition access_mapsto_def dq (m: gmap pid access) : iProp Σ := *)  (*   own (gen_access_name vmG) (◯ (map_fold (λ p a acc, *)  (*                                                      match a with *)  (*                                                        | NoAccess => acc *)  (*                                                        | SharedAccess => <[p:=(dq, (Cinl (to_agree ())))]>acc *)  (*                                                        | ExclusiveAccess => <[p:=(dq, (Cinr (Excl ())))]>acc *)  (*                                                      end) ∅ m)). *)  Definition access_mapsto_def (i:vmid) dq (s: gset_disj pid) : iProp Σ :=    own (gen_access_name vmG) (◯ {[i := (dq,  s)]}).  Definition access_mapsto_aux : seal (@access_mapsto_def). Proof. by eexists. Qed.  Definition access_mapsto := access_mapsto_aux.(unseal).  Definition access_mapsto_eq : @access_mapsto = @access_mapsto_def := access_mapsto_aux.(seal_eq).  Definition trans_mapsto_def(wh : word) dq (v: vmid) (wf: word) (wt: word) (pgs : gmap vmid (listset_nodup pid)) (fid : transaction_type) : iProp Σ :=    own (gen_trans_name vmG) (gmap_view_frag wh dq                          (((((v, wf) , wt), pgs), fid): (leibnizO (vmid * word * word * (gmap vmid (listset_nodup pid)) * transaction_type)))).  Definition trans_mapsto_aux : seal (@trans_mapsto_def). Proof. by eexists. Qed.  Definition trans_mapsto := trans_mapsto_aux.(unseal).  Definition trans_mapsto_eq : @trans_mapsto = @trans_mapsto_def := trans_mapsto_aux.(seal_eq).  Definition retri_mapsto_def (w:word) (s: gset_disj vmid) : iProp Σ :=    own (gen_retri_name vmG) (◯ {[w := s]}).  Definition retri_mapsto_aux : seal (@retri_mapsto_def). Proof. by eexists. Qed.  Definition retri_mapsto := retri_mapsto_aux.(unseal).  Definition retri_mapsto_eq : @retri_mapsto = @retri_mapsto_def := retri_mapsto_aux.(seal_eq).End definitions.(* predicate for the number of vms *)(* Notation "## n" := (num_agree n) *)(*                         (at level 50, format "## n"): bi_scope. *)(* predicate for current vm (token) *)Notation "<< n >>" := (token_agree n)                        (at level 50, format "<< n >>"): bi_scope.(* point-to predicates for registers and memory *)Notation "r @@ i ->r{ q } w" := (reg_mapsto r i (DfracOwn q) w)  (at level 22, q at level 50, format "r @@ i ->r{ q } w") : bi_scope.Notation "r @@ i ->r w" :=  (reg_mapsto r i (DfracOwn 1) w) (at level 21, w at level 50) : bi_scope.Notation "a ->a{ q } w" := (mem_mapsto a (DfracOwn q) w)  (at level 20, q at level 50, format "a ->a{ q } w") : bi_scope.Notation "a ->a w" := (mem_mapsto a (DfracOwn 1) w) (at level 20) : bi_scope.(* predicates for TX and RX *)Notation "TX@ i := p" := (tx_mapsto i p)                              (at level 20, format "TX@ i := p"): bi_scope.Notation "RX@ i :=( p ! n , r )" := (rx_mapsto1 i p (Some (n, r)))                                        (at level 20, format "RX@ i :=( p ! n , r )"):bi_scope.Notation "RX@ i :=( p !)" := (rx_mapsto1 i p None)                                        (at level 20, format "RX@ i :=( p !)"):bi_scope.Notation "RX@ i := p " := (rx_mapsto2 i p)                                        (at level 20, format "RX@ i := p"):bi_scope.(* predicates for pagetables *)Notation "O@ i :={ q }[ s ] " := (owned_mapsto i (DfracOwn q) (GSet s))                                           (at level 20, format "O@ i :={ q }[ s ] "):bi_scope.Notation "O@ i :={ q } p" := (owned_mapsto  i (DfracOwn q) (GSet {[p]}))                                           (at level 20, format "O@ i :={ q } p "):bi_scope.Notation "A@ i :={ q }[ s ] " := (access_mapsto i (DfracOwn q) (GSet s))                                          (at level 20, format "A@ i :={ q }[ s ] "):bi_scope.Notation "A@ i :={ q } p " := (access_mapsto  i (DfracOwn q) (GSet {[p]}))                                           (at level 20, format "A@ i :={ q } p "):bi_scope.(* predicates for transactions *)Notation "w ->t{ q }( v , x , y , m , f )" := (trans_mapsto w (DfracOwn q) v x y m f)                                                   (at level 20, format "w ->t{ q }( v , x , y , m , f )"):bi_scope.Notation "w ->re[ s ]" := (retri_mapsto w (GSet s))                              (at level 20, format "w ->re[ s ]"):bi_scope.Notation "w ->re v" := (retri_mapsto w (GSet {[v]}))                          (at level 20, format "w ->re v"):bi_scope.Section hyp_lang_rules.  Context `{vmG :!gen_VMG Σ}.  Implicit Types P Q : iProp Σ.  Implicit Types σ : state.  Implicit Types a b c : addr.  Implicit Types r : reg_name.  Implicit Types w: word.  Lemma token_valid i1 i2 :   << i1 >> -∗      << i2 >> -∗      ⌜ i1 = i2 ⌝.  Proof.    rewrite token_agree_eq /token_agree_def.    iIntros "H1 H2".    iDestruct (own_valid_2  with "H1 H2") as %Hvalid.    rewrite /get_token in Hvalid.    apply frac_agree_op_valid_L in Hvalid.    destruct Hvalid;done.   Qed.    Lemma token_update i1 i2 :   << i1 >> -∗      << i1 >> ==∗      << i2 >> ∗ << i2 >>.  Proof.    rewrite token_agree_eq /token_agree_def /get_token.    rewrite -own_op.    iApply own_update_2.    rewrite - frac_agree_op.    pose proof (to_frac_agree_exclusive (i1: leibnizO vmid)).    assert (Heq:  ( 1/2 + 1/2 =  1)%Qp ).    { apply (bool_decide_unpack _). by compute. }    rewrite Heq.    apply (cmra_update_exclusive ).    rewrite -frac_agree_op.    unfold to_frac_agree.    rewrite Heq.    apply pair_valid.    split;done.  Qed.  (* rules for register points-to *)  Lemma reg_dupl_false r i w1 w2 :   r @@ i ->r w1 -∗ r @@ i ->r w2 -∗ False.  Proof using.    rewrite reg_mapsto_eq /reg_mapsto_def.    iIntros "Hr1 Hr2".    iDestruct (ghost_map_elem_valid_2 with "Hr1 Hr2") as %?.    destruct H.    apply dfrac_valid_own_r in H.    inversion H.  Qed.  Lemma reg_neq r1 r2 i j w1 w2:   r1 @@ i ->r w1 -∗ r2 @@ j ->r w2 -∗ ⌜ r1 <> r2 ∨ i <> j⌝.  Proof using.    iIntros "Hr1 Hr2".    destruct (decide (r1 = r2)).    destruct (decide (i = j)).    - simplify_eq /=.      iDestruct (reg_dupl_false with "Hr1 Hr2") as %[].    - iRight. done.    - iLeft. done.  Qed.Lemma gen_reg_valid1:  ∀ (σ : state) r i w,    (get_current_vm σ) = i ->    ghost_map_auth (gen_reg_name vmG) 1 (get_reg_gmap σ) -∗    r @@ i ->r w -∗          ⌜ (get_reg σ r) = Some w ⌝.Proof.  iIntros (?????) "Hσ Hr".  rewrite reg_mapsto_eq /reg_mapsto_def.  iDestruct (ghost_map_lookup with "Hσ Hr") as "%".  iPureIntro.  rewrite /get_reg /get_reg_global.  unfold get_reg_gmap in H0.  apply elem_of_list_to_map_2 in H0.  apply elem_of_list_In in H0.  apply in_flat_map in H0.  inversion H0; clear H0.  destruct H1.  apply in_map_iff in H1.  inversion H1;clear H1.  inversion H2;clear H2.  inversion H1.  apply elem_of_list_In in H3.  apply elem_of_map_to_list' in H3.  by simplify_eq /=.Qed.(* TODO : quite ugly... *)Lemma gen_reg_valid_Sep:  ∀ (σ : state) i (regs: gmap (reg_name * vmid) word) ,    (get_current_vm σ) = i ->    ghost_map_auth (gen_reg_name vmG) 1 (get_reg_gmap σ) -∗    ([∗ map] r↦w ∈ regs,  r.1 @@ r.2 ->r w)-∗          ([∗ map] r↦w ∈ regs, ⌜r.2 = i -> (get_reg σ r.1) = Some w ⌝).Proof.  iIntros (????) "Hσ Hregs".  rewrite reg_mapsto_eq /reg_mapsto_def.  iDestruct ((ghost_map_lookup_big regs) with "Hσ [Hregs]") as "%Hincl".  iApply (big_sepM_proper (λ k x, (k.1, k.2)↪[gen_reg_name vmG] x)%I).  intros.  simplify_eq.  f_equiv.  by destruct k.  done.  iApply big_sepM_pure.  iIntros (????).  rewrite /get_reg /get_reg_global.  apply (lookup_weaken  _ (get_reg_gmap σ) _ _) in a1;eauto.  apply elem_of_list_to_map_2 in a1.  apply elem_of_list_In in a1.  apply in_flat_map in a1.  inversion a1; clear a1.  destruct H0.  apply in_map_iff in H1.  inversion H1;clear H1.  inversion H2;clear H2.  inversion H1.  apply elem_of_list_In in H3.  apply elem_of_map_to_list' in H3.  by simplify_eq /=.Qed.Lemma gen_reg_valid2:  ∀ (σ : state) i r1 w1 r2 w2 ,    (get_current_vm σ) = i ->    r1 ≠ r2->    ghost_map_auth (gen_reg_name vmG) 1 (get_reg_gmap σ) -∗                r1 @@ i ->r w1 -∗                             r2 @@ i ->r w2 -∗           ⌜ (get_reg σ r1) = Some w1 ⌝ ∗ ⌜ (get_reg σ r2) =Some w2 ⌝.Proof.  iIntros (?????? Hneq Hi) "Hreg Hr1 Hr2".  iDestruct ((gen_reg_valid_Sep σ i (<[(r1,i):=w1]>{[(r2,i):=w2]}))               with "Hreg [Hr1 Hr2]") as "%Hreg";eauto.  rewrite !big_sepM_insert ?big_sepM_empty;eauto.  iFrame.  apply lookup_insert_None; split;eauto; intros P; by inversion P.  iPureIntro.  split.  - by apply (Hreg (r1, i) w1 (lookup_insert _ (r1, i) w1)).  - apply (Hreg (r2, i) w2);eauto.    rewrite lookup_insert_Some;right;split;    [intros P; inversion P; contradiction|];    by rewrite !lookup_insert. Qed.Lemma gen_reg_valid3:  ∀ (σ : state) i r1 w1 r2 w2 r3 w3 ,    (get_current_vm σ) = i ->    r1 ≠ r2->    r1 ≠ r3->    r2 ≠ r3->    ghost_map_auth (gen_reg_name vmG) 1 (get_reg_gmap σ) -∗    r1 @@ i ->r w1 -∗    r2 @@ i ->r w2 -∗    r3 @@ i ->r w3 -∗                ⌜ (get_reg σ r1) = Some w1 ⌝ ∗ ⌜ (get_reg σ r2) =Some w2 ⌝ ∗ ⌜ (get_reg σ r3) = Some w3⌝.Proof.  iIntros (???????? Hi Hneq1 Hneq2 Hneq3) "Hreg Hr1 Hr2 Hr3".  iDestruct ((gen_reg_valid_Sep σ i ({[(r1,i):=w1;(r2,i):=w2;(r3,i):=w3]}))               with "Hreg [Hr1 Hr2 Hr3]") as "%Hreg";eauto.  rewrite !big_sepM_insert ?big_sepM_empty;eauto.  iFrame.  apply lookup_insert_None; split;eauto; intros P; by inversion P.  apply lookup_insert_None; split;eauto.  apply lookup_insert_None; split;eauto; intros P; by inversion P.  intros P; by inversion P.  iPureIntro.  split;[|split].  - by apply (Hreg (r1, i) w1 (lookup_insert _ (r1, i) w1)).  - apply (Hreg (r2, i) w2);eauto.    rewrite lookup_insert_Some;right;split;    [intros P; inversion P; contradiction|];    by rewrite !lookup_insert.  - apply (Hreg (r3, i) w3);eauto.    rewrite lookup_insert_Some;right;split;    [intros P; inversion P; contradiction|].    rewrite lookup_insert_Some;right;split;    [intros P; inversion P; contradiction|];    by rewrite !lookup_insert.Qed.Lemma gen_reg_update1_global:  ∀ (σ : state) r i w w',    ghost_map_auth (gen_reg_name vmG) 1 (get_reg_gmap σ) -∗    r @@ i ->r w ==∗               ghost_map_auth (gen_reg_name vmG) 1 (<[(r,i):=w']>(get_reg_gmap σ)) ∗              r @@ i ->r  w'. Proof.  iIntros (?????) "Hσ Hr".  rewrite reg_mapsto_eq /reg_mapsto_def.  iDestruct (ghost_map_update w' with "Hσ Hr") as ">[Hσ Hr]".  iFrame.  done. Qed. Lemma reg_proper {m: gmap (reg_name * vmid) word}:([∗ map] k ↦ x ∈ m, k↪[gen_reg_name vmG] x) ⊣⊢ ([∗ map]k ↦ x ∈ m,  (k.1, k.2)↪[gen_reg_name vmG] x).   Proof.      iApply (big_sepM_proper _ (λ k x, (k.1, k.2)↪[gen_reg_name vmG] x)%I).      intros.  simpl.  f_equiv.  destruct k;done.Qed. Lemma gen_reg_update_Sep:  ∀ (σ : state) regs regs',      dom (gset (reg_name * vmid)) regs = dom (gset (reg_name * vmid )) regs' ->    ghost_map_auth (gen_reg_name vmG) 1 (get_reg_gmap σ) -∗    ([∗ map] r↦w ∈ regs,  r.1 @@ r.2 ->r w) ==∗               ghost_map_auth (gen_reg_name vmG) 1 (regs' ∪ (get_reg_gmap σ)) ∗             ([∗ map] r↦w ∈ regs',  r.1 @@ r.2 ->r w). Proof.  iIntros (????) "Hσ Hr".  rewrite reg_mapsto_eq /reg_mapsto_def.  iDestruct (ghost_map_update_big regs regs' H with "[Hσ] [Hr]") as ">[Hσ Hr]".  done.  by iApply reg_proper.  iModIntro.  rewrite reg_proper.  iFrame. Qed. Lemma gen_reg_update2_global:  ∀ (σ : state) r1 i1 w1 w1' r2 i2 w2 w2',    r1 ≠ r2 ∨ i1 ≠ i2 ->    ghost_map_auth (gen_reg_name vmG) 1 (get_reg_gmap σ) -∗     r1 @@ i1 ->r w1 -∗                      r2 @@ i2 ->r w2==∗               ghost_map_auth (gen_reg_name vmG) 1 (<[(r1,i1) := w1']> (<[(r2,i2) := w2']> (get_reg_gmap σ))) ∗             r1 @@ i1 ->r w1'  ∗ r2 @@ i2 ->r w2'. Proof.  iIntros (????????? Hneq) "Hreg Hr1 Hr2".  iDestruct ((gen_reg_update_Sep _ {[(r1,i1):=w1; (r2,i2):=w2]} {[(r1,i1):=w1'; (r2,i2):=w2']}) with "Hreg [Hr1 Hr2]")    as ">[Hreg Hr12]" ;eauto;[set_solver| | ].        rewrite !big_sepM_insert ?big_sepM_empty;eauto.        iFrame.        destruct Hneq; apply lookup_insert_None; split;eauto; intros P; by inversion P.        iModIntro.        rewrite !big_sepM_insert ?big_sepM_empty;eauto.        iDestruct "Hr12" as "(? & ? & _)".        rewrite ?insert_union_singleton_l map_union_assoc.        simplify_map_eq.        by iFrame.        destruct Hneq; apply lookup_insert_None; split;eauto; intros P; by inversion P.Qed. (* rules for memory points-to *)  Lemma mem_dupl_false a w1 w2:   a ->a w1 -∗ a ->a w2 -∗ False.  Proof using.    rewrite mem_mapsto_eq /mem_mapsto_def.    iIntros "Ha1 Ha2".    iDestruct (ghost_map_elem_valid_2 with "Ha1 Ha2") as %?.    destruct H.    apply dfrac_valid_own_r in H.    inversion H.  Qed.  Lemma mem_neq a1 a2  w1 w2:   a1 ->a w1 -∗ a2 ->a w2 -∗ ⌜ a1 <> a2⌝.  Proof using.    iIntros "Ha1 Ha2".    destruct (decide (a1 = a2)).    - simplify_eq /=.      iDestruct (mem_dupl_false with "Ha1 Ha2") as %[].    - done.  Qed.Lemma gen_mem_valid:  ∀ (σ : state) a w,    ghost_map_auth (gen_mem_name vmG) 1 (get_mem σ) -∗    a ->a w -∗          ⌜ (get_mem σ) !! a = Some w ⌝.Proof.  iIntros (???) "Hσ Ha".  rewrite mem_mapsto_eq /mem_mapsto_def.  iDestruct (ghost_map_lookup with "Hσ Ha") as "%".  done. Qed.Lemma gen_mem_valid_Sep:  ∀ (σ : state) mem,    ghost_map_auth (gen_mem_name vmG) 1 (get_mem σ) -∗    ([∗ map] a↦w ∈ mem,  a ->a w)-∗         ([∗ map] a↦w ∈ mem, ⌜ (get_mem σ) !! a = Some w ⌝).Proof.  iIntros (??) "Hσ Hmem".  rewrite mem_mapsto_eq /mem_mapsto_def.  iDestruct ((ghost_map_lookup_big mem) with "Hσ Hmem") as "%Hincl".  iApply big_sepM_pure.  iIntros (???).  iPureIntro.  apply (lookup_weaken  mem (get_mem σ) _ _ a1 Hincl) .Qed.Lemma gen_mem_valid2:  ∀ (σ : state) a1 w1 a2 w2,    a1 ≠ a2 ->    ghost_map_auth (gen_mem_name vmG) 1 (get_mem σ) -∗    a1 ->a w1 -∗    a2 ->a w2 -∗          ⌜ (get_mem σ) !! a1 = Some w1 ⌝ ∗ ⌜ (get_mem σ) !! a2 = Some w2 ⌝.Proof.  iIntros (????? Hneq) "Hσ Ha1 Ha2".  iDestruct (gen_mem_valid_Sep _ {[a1:=w1;a2:=w2]} with "Hσ [Ha1 Ha2]") as "%";eauto.  rewrite !big_sepM_insert ?big_sepM_empty;eauto.  iFrame.  by simplify_map_eq.  iPureIntro.  split.  - by apply (H a1 w1 (lookup_insert _ a1 w1)).  - apply (H a2 w2);eauto.    by simplify_map_eq. Qed.Lemma gen_mem_update1:  ∀ (σ : state) a w w',    ghost_map_auth (gen_mem_name vmG) 1 (get_mem σ) -∗    a ->a w ==∗               ghost_map_auth (gen_mem_name vmG) 1 (<[a:=w']>(get_mem σ)) ∗              a ->a w'. Proof.  iIntros (????) "Hσ Ha".  rewrite mem_mapsto_eq /mem_mapsto_def.  iDestruct (ghost_map_update w' with "Hσ Ha") as ">[Hσ Ha]".  iFrame.  done. Qed. (* rules for TX *)  Lemma tx_dupl i p :   TX@ i := p -∗ TX@ i := p ∗ TX@ i := p.  Proof using.    rewrite tx_mapsto_eq.    iIntros "Htx".    iApply own_op.    rewrite -auth_frag_op singleton_op.    rewrite agree_idemp.    done.  Qed.  Lemma gen_tx_valid σ i p:   TX@ i := p -∗ own (gen_tx_name vmG) (get_tx_agree σ) -∗ ⌜ (get_vm_mail_box σ i).1 = p ⌝.  Proof.    iIntros "Htx Hσ".    rewrite tx_mapsto_eq /mem_mapsto_def.    Admitted.  (* rules for RX *)  Lemma rx_split_some i p n (v: vmid):  RX@ i :=( p ! n , v)  -∗ RX@ i :=( p ! n, v)  ∗ RX@ i := p.  Proof using.    iIntros "HR".    rewrite rx_mapsto_eq1 rx_mapsto_eq2.    iApply own_op.    rewrite -pair_op -auth_frag_op.    rewrite singleton_op agree_idemp.    rewrite Some_op_opM.    simplify_eq /=.    done.  Qed.  Lemma rx_split_none i p:  RX@ i :=(p !) -∗ RX@ i :=(p !) ∗ RX@ i := p.  Proof using.    iIntros "HR".    rewrite rx_mapsto_eq1 rx_mapsto_eq2.    iApply own_op.    rewrite -pair_op -auth_frag_op.    rewrite singleton_op agree_idemp.    rewrite  Some_op_opM.    simplify_eq /=.    done.  Qed.  Lemma rx_dupl i p:   RX@i:=p -∗ RX@i:=p ∗ RX@i:=p.  Proof using.    iIntros "HR".    rewrite rx_mapsto_eq2.    iApply own_op.    rewrite -pair_op -auth_frag_op.    rewrite singleton_op agree_idemp.    naive_solver.  Qed.  Lemma gen_rx_agree_valid σ i p:   ✓ (get_rx_agree σ ⋅ ◯ {[i := to_agree p]}) -> (get_vm_mail_box σ i).2.1 = p.  Proof.    intro.    rewrite /get_rx_agree /get_txrx_auth_agree in H.    apply auth_both_valid_discrete in H;destruct H as [H _].    remember  ((list_to_map (map (λ v : vmid, (v, to_agree (get_vm_mail_box σ v).2.1)) list_of_vmids)): gmap vmid (agreeR (leibnizO pid))) as m.    rewrite -Heqm in H.    rewrite -> (lookup_included {[i := to_agree p]} m) in H.    pose proof (H i).    clear H.    simplify_map_eq /=.    apply option_included_total in H0;destruct H0.    rewrite -> (lookup_singleton_None i i (to_agree p)) in H;done.    destruct H as [x [x0 [H H0]]].    rewrite -> (lookup_singleton_Some i i (to_agree p)) in H.    inversion H; subst x;clear H H1.    destruct H0.    apply elem_of_list_to_map_2 in H.    apply elem_of_list_In in H.    apply in_map_iff in H.    inversion H;clear H.    destruct H1 as [H1 _];inversion H1;subst;clear H1.    rewrite -> (to_agree_included (p: (leibnizO pid)) _) in H0.    by fold_leibniz.  Qed.  Lemma gen_rx_pid_valid σ i p:   RX@ i := p -∗ own (gen_rx_name vmG) ((get_rx_agree σ), (get_rx_gmap σ) )-∗ ⌜ (get_vm_mail_box σ i).2.1 = p ⌝.  Proof.    iIntros "Hrx Hσ".    rewrite rx_mapsto_eq2 /rx_mapsto_def2 .    iDestruct (own_valid_2  with "Hσ Hrx") as %?.    iPureIntro.    rewrite -pair_op in H.    apply pair_valid in H; destruct H as [H _].    simpl in H.    by apply gen_rx_agree_valid.  Qed.  Lemma gen_rx_gmap_none_valid σ i:  ✓ (get_rx_gmap σ ⋅ Some (gmap_view_frag i (DfracOwn 1) None)) -> (get_vm_mail_box σ i).2.2 = None.  Proof.    intro.    rewrite /get_rx_gmap -Some_op in H.    rewrite -> Some_valid in H.    apply gmap_view_both_frac_valid_L in H as [_ [_ H]].    apply elem_of_list_to_map_2 in H.    apply elem_of_list_In in H.    apply in_map_iff in H.    destruct H as [x [H _]].    destruct ((get_vm_mail_box σ x).2.2) eqn:Heqn.    destruct p;inversion H.    inversion H;subst.    by inversion H.  Qed.  Lemma gen_rx_none_valid σ i p:   RX@ i :=( p !) -∗   own (gen_rx_name vmG) ((get_rx_agree σ), (get_rx_gmap σ) )-∗   ⌜ (get_vm_mail_box σ i).2 = (p,None)  ⌝.  Proof.    iIntros "Hrx Hσ".    rewrite rx_mapsto_eq1 /rx_mapsto_def1.    iDestruct (own_valid_2 with "Hσ Hrx") as %?.    iPureIntro.    rewrite -pair_op in H.    apply pair_valid in H; destruct H as [Hagree Hgmap];simpl in Hagree;simpl in Hgmap.    apply gen_rx_agree_valid in Hagree.    apply gen_rx_gmap_none_valid in Hgmap.    destruct ((get_vm_mail_box σ i).2) eqn:Heqn.    rewrite -Hagree -Hgmap.    done.  Qed.  Lemma gen_rx_gmap_some_valid σ i l v:  ✓ (get_rx_gmap σ ⋅ Some (gmap_view_frag i (DfracOwn 1) (Some(l,v)))) -> (get_vm_mail_box σ i).2.2 = Some(l,v).  Proof.    intro.    rewrite /get_rx_gmap -Some_op in H.    rewrite -> Some_valid in H.    apply gmap_view_both_frac_valid_L in H as [_ [_ H]].    apply elem_of_list_to_map_2 in H.    apply elem_of_list_In in H.    apply in_map_iff in H.    destruct H as [x [H _]].    destruct ((get_vm_mail_box σ x).2.2) eqn:Heqn.    by destruct p;inversion H;subst.    by inversion H.  Qed.  Lemma gen_rx_valid_some σ i p l v:   RX@ i :=( p ! l , v) -∗   own (gen_rx_name vmG) ((get_rx_agree σ), (get_rx_gmap σ) )-∗   ⌜ (get_vm_mail_box σ i).2 = (p,Some(l,v))⌝.  Proof.    iIntros "Hrx Hσ".    rewrite rx_mapsto_eq1 /rx_mapsto_def1.    iDestruct (own_valid_2 with "Hσ Hrx") as %?.    iPureIntro.    rewrite -pair_op in H.    apply pair_valid in H; destruct H as [Hagree Hgmap];simpl in Hagree;simpl in Hgmap.    apply gen_rx_agree_valid in Hagree.    apply gen_rx_gmap_some_valid in Hgmap.    destruct ((get_vm_mail_box σ i).2) eqn:Heqn.    rewrite -Hagree -Hgmap.    done.  Qed.  (* rules for pagetables  *)  Lemma owned_split_set i q1 q2 (s1 s2 : gset pid):   s1 ## s2 -> O@i:={(q1+q2)%Qp}[(s1 ∪ s2)] -∗ O@i:={q1}[s1] ∗ O@i:={q2}[s2].  Proof using.  iIntros (Hdisj) "HO".  rewrite owned_mapsto_eq.  iApply own_op.  rewrite -auth_frag_op singleton_op.  rewrite -pair_op.  rewrite (gset_disj_union _ _ Hdisj).  naive_solver.  Qed.  Lemma owned_split_singleton i q1 q2 (s : gset pid) p:   p ∉ s -> O@i:={(q1+q2)%Qp}[(s ∪ {[p]})] -∗ O@i:={q1}[s] ∗ O@i:={q2}p.  Proof using.    iIntros (Hnotin) "HO".    assert (Hdisj: s ## {[p]}). { set_solver. }    iDestruct (owned_split_set i q1 q2 _ _ Hdisj with "HO")  as "HO'".    done.  Qed. Lemma access_split_set i q1 q2 (s1 s2 : gset pid):   s1 ## s2 -> A@i:={(q1+q2)%Qp}[(s1 ∪ s2)] -∗ A@i:={q1}[s1] ∗ A@i:={q2}[s2].  Proof using.  iIntros (Hdisj) "HO".  rewrite access_mapsto_eq.  iApply own_op.  rewrite -auth_frag_op singleton_op.  rewrite -pair_op.  rewrite (gset_disj_union _ _ Hdisj).  naive_solver.  Qed.  Lemma access_split_singleton i q1 q2 (s : gset pid) p:   p ∉ s -> A@i:={(q1+q2)%Qp}[(s ∪ {[p]})] -∗ A@i:={q1}[s] ∗ A@i:={q2}p.  Proof using.    iIntros (Hnotin) "HO".    assert (Hdisj: s ## {[p]}). { set_solver. }    iDestruct (access_split_set i q1 q2 _ _ Hdisj with "HO")  as "HO'".    done.  Qed.Lemma gen_access_valid_Set:  ∀ (σ : state) i q (s:gset pid),    own (gen_access_name vmG) (get_access_gmap σ)  -∗    (A@ i :={q}[s] ) -∗          ([∗ set]  p ∈ s, ⌜(check_access_page σ i p)= true ⌝).Proof.    iIntros (????) "Hσ Hacc".    rewrite access_mapsto_eq /access_mapsto_def.    iDestruct (own_valid_2 with "Hσ Hacc") as %Hvalid.    iPureIntro.    unfold get_access_gmap in Hvalid.    apply auth_both_valid_discrete in Hvalid.    destruct Hvalid.    remember (list_to_map (map              (λ v : vmid,                 (v,                 (DfracOwn 1,                 GSet                   (list_to_set                      (map (λ p : pid * permission, p.1)                         (map_to_list                            (filter (λ p : pid * permission, is_accessible p.2 = true)                               (get_vm_page_table σ v)))))))) list_of_vmids)) as m.    pose proof (lookup_included {[i := (DfracOwn q, GSet s)]} m).    rewrite ->H1 in H.    clear H1.    pose proof (H i).    clear H.    apply option_included in H1.    destruct H1.    simplify_map_eq.    destruct H.    destruct H.    destruct H.    apply lookup_singleton_Some in H.    destruct H.   simplify_map_eq /=.    destruct H1.   apply (elem_of_list_to_map_2 _ i x0) in H.   apply elem_of_list_In in H.   apply (in_map_iff ) in H.   destruct H.   destruct H.   inversion H.   simplify_eq /=.   clear H.   unfold set_Forall.   intros p Hin.   destruct H1.  - inversion H;clear H.      simplify_eq /=.      unfold check_access_page.      apply elem_of_list_to_set in Hin.      apply elem_of_list_In in Hin.      apply (in_map_iff _ _ p) in Hin.      destruct Hin.      destruct H.      rewrite <- elem_of_list_In in H1.      apply elem_of_map_to_list' in H1.      apply map_filter_lookup_Some in H1.      destruct H1.      subst p.      by rewrite H1 /=.    - apply pair_included in H.      destruct H;clear H.      apply gset_disj_included in H1.      unfold check_access_page.      assert ( p ∈ (list_to_set           (map (λ p : pid * permission, p.1)              (map_to_list (filter (λ p : pid * permission, is_accessible p.2 = true) (get_vm_page_table σ i)))): gset pid)) as Hin'.      { set_solver.  }      clear Hin;rename Hin' into Hin.      apply elem_of_list_to_set in Hin.      apply elem_of_list_In in Hin.      apply (in_map_iff _ _ p) in Hin.      destruct Hin.      destruct H.      rewrite <- elem_of_list_In in H3.      apply elem_of_map_to_list' in H3.      apply map_filter_lookup_Some in H3.      destruct H3.      subst p.      rewrite H3.      done.Qed.  Lemma gen_access_valid:  ∀ (σ : state) i q p,    own (gen_access_name vmG) (get_access_gmap σ)  -∗    (A@ i :={q}p ) -∗          ( ⌜(check_access_page σ i p)= true ⌝).  Proof.     iIntros (????) "Hσ Hacc".     iDestruct (gen_access_valid_Set _ _ _ {[p]} with "Hσ Hacc") as %->;eauto.     set_solver.  Qed.Lemma gen_access_valid_addr:  ∀ (σ : state) i q a,    own (gen_access_name vmG) (get_access_gmap σ)  -∗    (A@ i :={q} (mm_translation a) ) -∗          ( ⌜(check_access_addr σ i a)= true ⌝).Proof.  iIntros (????) "Haccess Hacc".  iDestruct (gen_access_valid σ i q (mm_translation a) with "Haccess Hacc") as %Hacc.  iPureIntro.  by unfold check_access_page.Qed.Lemma gen_access_valid_addr2:  ∀ (σ : state) i q s a1 a2,      s= {[(mm_translation a1); (mm_translation a2)]} ->    own (gen_access_name vmG) (get_access_gmap σ)  -∗    (A@ i :={q}[s] ) -∗          ( ⌜(check_access_addr σ i a1)= true ⌝ ∗ ⌜(check_access_addr σ i a2)= true ⌝).Proof.  iIntros (???????) "Haccess Hacc".  iDestruct (gen_access_valid_Set σ i q s with "Haccess Hacc") as %Hacc.  iPureIntro.  split.  pose proof (Hacc (mm_translation a1)).  apply H0.  set_solver.  pose proof (Hacc (mm_translation a2)).  apply H0.  set_solver.Qed.  (* TODO : gen_access_valid_Sep*)  (* rules for transactions *)  Lemma trans_split wh q1 q2 i wf wt m f:   wh ->t{(q1+q2)%Qp}(i,wf,wt,m,f) -∗  wh ->t{q1}(i,wf,wt,m,f) ∗ wh ->t{q2}(i,wf,wt,m,f).  Proof using.    iIntros "HT".    rewrite trans_mapsto_eq.    iApply own_op.    rewrite -gmap_view_frag_op.    rewrite dfrac_op_own.    done.  Qed.  Lemma retri_split_set wh (s1 s2 : gset vmid):   s1 ## s2 -> wh ->re[(s1 ∪ s2)] -∗ wh ->re[s1] ∗ wh ->re[s2].  Proof using.    iIntros (Hdisj) "Hre".    rewrite retri_mapsto_eq.    iApply own_op.    rewrite -auth_frag_op singleton_op.    rewrite (gset_disj_union _ _ Hdisj).    naive_solver.  Qed.  Lemma  retri_split_singleton wh (s: gset vmid) i:   i ∉ s -> wh ->re[(s ∪ {[i]})] -∗ wh ->re[s] ∗ wh ->re i.  Proof using.    iIntros (Hnotin) "Hr".    assert (Hdisj: s ## {[i]}).    { set_solver. }    iDestruct (retri_split_set wh _ _ Hdisj with "Hr")  as "Hr'".    done.  Qed.End hyp_lang_rules.
