theories/rules.v
@@ -361,5 +361,59 @@ Proof.
       apply (get_reg_gmap_get_reg_Some _ _ _ i) in HPC;eauto.
 Qed.
 
+Lemma str_eq {i w1 w2 q s instr} ai a ra:
+  instr = Str ra ra ->
+  decode_instruction w1 = Some(instr) ->
+  PC ≠ ra ->
+  NZ ≠ ra ->
+  ai ≠ a ->
+  s = {[(mm_translation ai);(mm_translation a)]} ->
+  <<i>> ∗ PC @@ i ->r ai ∗ ai ->a w1 ∗ ra @@ i ->r a ∗ a ->a w2 ∗ A@i:={q}[s]
+    ⊢ SSWP ExecI @ i {{ (λ m, ⌜m = ExecI ⌝ ∗ <<i>> ∗ PC @@ i ->r (ai +w 1) ∗ ai ->a w1 ∗ ra @@ i ->r a ∗ a ->a a
+                                      ∗ A@i:={q}[s]) }}%I.
+Proof.
+  iIntros (Hinstr Hdecode HneqPCa HneqNZa HneqPCb HneqNZb Hneqab Hneqaia Hs) "(? & Hpc & Hapc & Hrb & Harb & Hacc & Hra )".
+  iApply (sswp_lift_atomic_step ExecI);[done|].
+  iIntros (σ1) "%Hsche Hσ".
+  inversion Hsche as [ Hcur ]; clear Hsche.
+  apply fin_to_nat_inj in Hcur.
+  iModIntro.
+  iDestruct "Hσ" as "(? & Hmem & Hreg & ? & ? & ? & Haccess & ?)".
+  (* valid regs *)
+  iDestruct ((gen_reg_valid3 σ1 i PC ai ra w2 rb a Hcur HneqPCa HneqPCb Hneqab ) with "Hreg Hpc Hra Hrb") as "[%HPC [%Hra %Hrb]]".
+  (* valid pt *)
+  iDestruct ((gen_access_valid_addr2 σ1 i q s ai a Hs) with "Haccess Hacc") as "[%Hai %Ha]".
+  (* valid mem *)
+  iDestruct (gen_mem_valid2 σ1 ai w1 a w3 Hneqaia with "Hmem Hapc Harb ") as "[%Hmemai %Hmema]".
+  iSplit.
+  - (* reducible *)
+    iPureIntro.
+    apply (reducible_normal i instr ai w1);eauto.
+  - (* step *)
+    iModIntro.
+    iIntros (m2 σ2) "%HstepP".
+    apply (step_ExecI_normal i instr ai w1 ) in HstepP;eauto.
+    remember (exec instr σ1) as c2 eqn:Heqc2.
+    rewrite /exec Hinstr (str_ExecI σ1 ra rb w2 a HneqPCa HneqNZa HneqPCb HneqNZb Hra Hrb) /update_incr_PC in Heqc2.
+    2: {
+       by rewrite Hcur Ha.
+    }
+    destruct HstepP;subst m2 σ2; subst c2; simpl.
+    rewrite /gen_vm_interp.
+    (* unchanged part *)
+    rewrite_reg_all.
+    rewrite Hcur.
+    iFrame.
+    (* updated part *)
+    rewrite -> (update_offset_PC_update_PC1 _ i ai 1);eauto.
+    + rewrite update_memory_unsafe_preserve_reg.
+      iDestruct ((gen_reg_update1_global σ1 PC i ai (ai +w 1)) with "Hreg Hpc") as ">[Hreg Hpc]";eauto.
+      iDestruct ((gen_mem_update1 σ1 a w3 w2) with "Hmem Harb") as ">[Hmem Harb]";eauto.
+      rewrite (update_memory_unsafe_update_mem σ1 a w2);eauto.
+      by iFrame.
+    + rewrite update_memory_unsafe_preserve_reg.
+      apply (get_reg_gmap_get_reg_Some _ _ _ i) in HPC;eauto.
+Qed.
+
 
 End rules.
